Add doc comments to AtomsAndFacts

ExistentialRules/AtomsAndFacts/Basic.lean
@@ -6,335 +6,458 @@ import BasicLeanDatastructures.Set.Finite
 import ExistentialRules.Terms.Basic
 import ExistentialRules.Terms.ListsOfTerms
 
-section StructuralDefs
+/-!
+# Atoms, Facts, Rules and the like
 
-  structure GeneralizedAtom (sig : Signature) (T : Type u) [DecidableEq sig.P] where
-    predicate : sig.P
-    terms : List T
-    arity_ok : terms.length = sig.arity predicate
-    deriving DecidableEq
+In this file, we define the next layers of building blocks above terms.
+This includes first and foremost `Atom` and `Fact` but also
+`Rule`, `RuleSet`, `Database` and `KnowledgeBase` to name a few.
 
-  abbrev FunctionFreeFact (sig : Signature) [DecidableEq sig.P] := GeneralizedAtom sig sig.C
-  abbrev Fact (sig : Signature) [DecidableEq sig.P] [DecidableEq sig.C] [DecidableEq sig.V] := GeneralizedAtom sig (GroundTerm sig)
-  abbrev FunctionFreeAtom (sig : Signature) [DecidableEq sig.P] [DecidableEq sig.C] [DecidableEq sig.V] := GeneralizedAtom sig (VarOrConst sig)
-  abbrev Atom (sig : Signature) [DecidableEq sig.P] [DecidableEq sig.C] [DecidableEq sig.V] := GeneralizedAtom sig (SkolemTerm sig)
+The atom-like datastructures are all expressed in terms of a `GeneralizedAtom`. This will turn out convenient when defining substitutions and homomorphisms next since these can (for the most part) just be defines as generic mapping over `GeneralizedAtom`.
+-/
 
-  variable (sig : Signature) [DecidableEq sig.P] [DecidableEq sig.C] [DecidableEq sig.V]
+/-- A `GeneralizedAtom` consists of a predicate symbol and a list of terms of an arbitrary type such that the number of terms matches the predicate's arity. -/
+structure GeneralizedAtom (sig : Signature) (T : Type u) [DecidableEq sig.P] where
+  predicate : sig.P
+  terms : List T
+  arity_ok : terms.length = sig.arity predicate
+deriving DecidableEq
 
-  abbrev FunctionFreeConjunction := List (FunctionFreeAtom sig)
+/-!
+## Atom
+-/
 
-  -- normally, we would only allow variables in atoms in rules... does this break later?
-  structure Rule where
-    id : Nat
-    body : FunctionFreeConjunction sig
-    head : List (FunctionFreeConjunction sig)
-    deriving DecidableEq
+/-- An `Atom` is a `GeneralizedAtom` with `SkolemTerm`s. -/
+abbrev Atom (sig : Signature) [DecidableEq sig.P] [DecidableEq sig.C] [DecidableEq sig.V] := GeneralizedAtom sig (SkolemTerm sig)
 
-  structure RuleSet where
-    rules : Set (Rule sig)
-    id_unique : ∀ r1 r2, r1 ∈ rules ∧ r2 ∈ rules ∧ r1.id = r2.id -> r1 = r2
+section FunctionFreeAtom
 
-  structure RuleList where
-    rules : List (Rule sig)
-    id_unique : ∀ r1 r2, r1 ∈ rules ∧ r2 ∈ rules ∧ r1.id = r2.id -> r1 = r2
+/-!
+## FunctionFreeAtom
+-/
 
-  abbrev FactSet := Set (Fact sig)
-
-  abbrev Database := { X : Set (FunctionFreeFact sig) // X.finite }
-
-  structure KnowledgeBase where
-    db : Database sig
-    rules : RuleSet sig
-
-end StructuralDefs
-
-
-variable {sig : Signature} [DecidableEq sig.P] [DecidableEq sig.C] [DecidableEq sig.V]
+/-- A `FunctionFreeAtom` is a `GeneralizedAtom` with `VarOrConst`s. -/
+abbrev FunctionFreeAtom (sig : Signature) [DecidableEq sig.P] [DecidableEq sig.C] [DecidableEq sig.V] := GeneralizedAtom sig (VarOrConst sig)
 
 namespace FunctionFreeAtom
 
-  def variables (a : FunctionFreeAtom sig) : List sig.V := VarOrConst.filterVars a.terms
+variable {sig : Signature} [DecidableEq sig.P] [DecidableEq sig.C] [DecidableEq sig.V]
 
-  def constants (a : FunctionFreeAtom sig) : List sig.C := VarOrConst.filterConsts a.terms
+/-- Using `VarOrConst.filterVars`, we can obtain all variables from the terms of the `FunctionFreeAtom`. -/
+def variables (a : FunctionFreeAtom sig) : List sig.V := VarOrConst.filterVars a.terms
 
-  def skolemize (ruleId : Nat) (disjunctIndex : Nat) (frontier : List sig.V) (a : FunctionFreeAtom sig) : Atom sig := {
-    predicate := a.predicate,
-    terms := a.terms.map (VarOrConst.skolemize ruleId disjunctIndex frontier),
-    arity_ok := by rw [List.length_map, a.arity_ok]
-  }
+/-- Using `VarOrConst.filterConsts`, we can obtain all constants from the terms of the `FunctionFreeAtom`. -/
+def constants (a : FunctionFreeAtom sig) : List sig.C := VarOrConst.filterConsts a.terms
 
-  theorem mem_variables {a : FunctionFreeAtom sig} {v : sig.V} : v ∈ a.variables ↔ (VarOrConst.var v) ∈ a.terms := by
-    constructor
-    . intro v_mem; apply VarOrConst.filterVars_occur_in_original_list; exact v_mem
-    . intro v_mem; apply VarOrConst.mem_filterVars_of_var; exact v_mem
+/-- We can `skolemize` a `FunctionFreeAtom` by skolemizing all its `VarOrConst`s. This yields an `Atom`. -/
+def skolemize (ruleId : Nat) (disjunctIndex : Nat) (frontier : List sig.V) (a : FunctionFreeAtom sig) : Atom sig := {
+  predicate := a.predicate,
+  terms := a.terms.map (VarOrConst.skolemize ruleId disjunctIndex frontier),
+  arity_ok := by rw [List.length_map, a.arity_ok]
+}
 
-  theorem mem_constants {a : FunctionFreeAtom sig} {c : sig.C} : c ∈ a.constants ↔ (VarOrConst.const c) ∈ a.terms := by
-    constructor
-    . intro c_mem; apply VarOrConst.filterConsts_occur_in_original_list; exact c_mem
-    . intro c_mem; apply VarOrConst.mem_filterConsts_of_const; exact c_mem
+/-- A variable occurs in `variables` iff it is a term of the `FunctionFreeAtom. -/
+theorem mem_variables {a : FunctionFreeAtom sig} {v : sig.V} : v ∈ a.variables ↔ (VarOrConst.var v) ∈ a.terms := by
+  constructor
+  . intro v_mem; apply VarOrConst.filterVars_occur_in_original_list; exact v_mem
+  . intro v_mem; apply VarOrConst.mem_filterVars_of_var; exact v_mem
 
-  theorem length_skolemize {ruleId : Nat} {disjunctIndex : Nat} {frontier : List sig.V} {a : FunctionFreeAtom sig} :
-      (a.skolemize ruleId disjunctIndex frontier).terms.length = a.terms.length := by
-    unfold skolemize
-    rw [List.length_map]
+/-- A constant occurs in `constants` iff it is a term of the `FunctionFreeAtom. -/
+theorem mem_constants {a : FunctionFreeAtom sig} {c : sig.C} : c ∈ a.constants ↔ (VarOrConst.const c) ∈ a.terms := by
+  constructor
+  . intro c_mem; apply VarOrConst.filterConsts_occur_in_original_list; exact c_mem
+  . intro c_mem; apply VarOrConst.mem_filterConsts_of_const; exact c_mem
 
-  theorem mem_skolemize_of_mem {ruleId : Nat} {disjunctIndex : Nat} {frontier : List sig.V}
-      {a : FunctionFreeAtom sig} {t : VarOrConst sig} :
-      t ∈ a.terms -> (t.skolemize ruleId disjunctIndex frontier) ∈ (a.skolemize ruleId disjunctIndex frontier).terms := by
-    intro t_mem
-    unfold skolemize
-    rw [List.mem_map]
-    exists t
+/-- The number of terms remains unchanged when Skolemizing. -/
+theorem length_skolemize {ruleId : Nat} {disjunctIndex : Nat} {frontier : List sig.V} {a : FunctionFreeAtom sig} :
+    (a.skolemize ruleId disjunctIndex frontier).terms.length = a.terms.length := by
+  unfold skolemize
+  rw [List.length_map]
+
+/-- If a a `VarOrConst` occurs in the terms of the `FunctionFreeAtom`, then the Skolemized `VarOrConst` occurs in the Skolemized `Atom`. -/
+theorem mem_skolemize_of_mem {ruleId : Nat} {disjunctIndex : Nat} {frontier : List sig.V}
+    {a : FunctionFreeAtom sig} {t : VarOrConst sig} :
+    t ∈ a.terms -> (t.skolemize ruleId disjunctIndex frontier) ∈ (a.skolemize ruleId disjunctIndex frontier).terms := by
+  intro t_mem
+  unfold skolemize
+  rw [List.mem_map]
+  exists t
 
 end FunctionFreeAtom
 
+end FunctionFreeAtom
+
+section FunctionFreeConjunction
+
+/-!
+## FunctionFreeConjunction
+-/
+
+/-- A conjunction of `FunctionFreeAtom`s $p(x, y) \land q(y)$ can simply be represented as a list of `FunctionFreeAtom`s. -/
+abbrev FunctionFreeConjunction (sig : Signature) [DecidableEq sig.P] [DecidableEq sig.C] [DecidableEq sig.V] := List (FunctionFreeAtom sig)
+
 namespace FunctionFreeConjunction
 
-  def terms (conj : FunctionFreeConjunction sig) : List (VarOrConst sig) := conj.flatMap GeneralizedAtom.terms
+variable {sig : Signature} [DecidableEq sig.P] [DecidableEq sig.C] [DecidableEq sig.V]
 
-  def vars (conj : FunctionFreeConjunction sig) : List sig.V := conj.flatMap FunctionFreeAtom.variables
+/-- The `terms` of a `FunctionFreeConjunction` are the terms of all its atoms. -/
+def terms (conj : FunctionFreeConjunction sig) : List (VarOrConst sig) := conj.flatMap GeneralizedAtom.terms
 
-  def consts (conj : FunctionFreeConjunction sig) : List sig.C := conj.flatMap FunctionFreeAtom.constants
+/-- The `vars` of a `FunctionFreeConjunction` are the variables of all its atoms. -/
+def vars (conj : FunctionFreeConjunction sig) : List sig.V := conj.flatMap FunctionFreeAtom.variables
 
-  def predicates (conj : FunctionFreeConjunction sig) : List sig.P := conj.map GeneralizedAtom.predicate
+/-- The `consts` of a `FunctionFreeConjunction` are the constants of all its atoms. -/
+def consts (conj : FunctionFreeConjunction sig) : List sig.C := conj.flatMap FunctionFreeAtom.constants
 
-  theorem mem_vars {conj : FunctionFreeConjunction sig} {v : sig.V} :
-      v ∈ conj.vars ↔ ∃ f, f ∈ conj ∧ (VarOrConst.var v) ∈ f.terms := by
-    unfold vars; rw [List.mem_flatMap]
-    constructor
-    . rintro ⟨f, f_mem, v_mem⟩; exists f; constructor; exact f_mem; rw [← FunctionFreeAtom.mem_variables]; exact v_mem
-    . rintro ⟨f, f_mem, v_mem⟩; exists f; constructor; exact f_mem; rw [FunctionFreeAtom.mem_variables]; exact v_mem
+/-- The `predicates` of a `FunctionFreeConjunction` are the predicates of all its atoms. -/
+def predicates (conj : FunctionFreeConjunction sig) : List sig.P := conj.map GeneralizedAtom.predicate
 
-  theorem mem_consts {conj : FunctionFreeConjunction sig} {c : sig.C} :
-      c ∈ conj.consts ↔ ∃ f, f ∈ conj ∧ (VarOrConst.const c) ∈ f.terms := by
-    unfold consts; rw [List.mem_flatMap]
-    constructor
-    . rintro ⟨f, f_mem, c_mem⟩; exists f; constructor; exact f_mem; rw [← FunctionFreeAtom.mem_constants]; exact c_mem
-    . rintro ⟨f, f_mem, c_mem⟩; exists f; constructor; exact f_mem; rw [FunctionFreeAtom.mem_constants]; exact c_mem
+/-- Different from the definition, we can also say that a variable is in `variables` iff there is a `FunctionFreeAtom` in the conjunction that features the variable as a term. -/
+theorem mem_vars {conj : FunctionFreeConjunction sig} {v : sig.V} :
+    v ∈ conj.vars ↔ ∃ f, f ∈ conj ∧ (VarOrConst.var v) ∈ f.terms := by
+  unfold vars; rw [List.mem_flatMap]
+  constructor
+  . rintro ⟨f, f_mem, v_mem⟩; exists f; constructor; exact f_mem; rw [← FunctionFreeAtom.mem_variables]; exact v_mem
+  . rintro ⟨f, f_mem, v_mem⟩; exists f; constructor; exact f_mem; rw [FunctionFreeAtom.mem_variables]; exact v_mem
+
+/-- Different from the definition, we can also say that a constant is in `constants` iff there is a `FunctionFreeAtom` in the conjunction that features the constant as a term. -/
+theorem mem_consts {conj : FunctionFreeConjunction sig} {c : sig.C} :
+    c ∈ conj.consts ↔ ∃ f, f ∈ conj ∧ (VarOrConst.const c) ∈ f.terms := by
+  unfold consts; rw [List.mem_flatMap]
+  constructor
+  . rintro ⟨f, f_mem, c_mem⟩; exists f; constructor; exact f_mem; rw [← FunctionFreeAtom.mem_constants]; exact c_mem
+  . rintro ⟨f, f_mem, c_mem⟩; exists f; constructor; exact f_mem; rw [FunctionFreeAtom.mem_constants]; exact c_mem
 
 end FunctionFreeConjunction
 
+end FunctionFreeConjunction
+
+section Rule
+
+/-!
+## (Disjunctive) (Existential) Rule
+
+A disjunctive existential rule, or simply `Rule`, formally is an expression of the form
+$$∀ \vec{x}, \vec{y}. B(x, y) \to \bigvee_{i = 1}^{k} \exists \vec{z}_i. H_i(y_i, z_i)$$
+where $B,H_1,\dots,H_k$ are conjunctions of function free atoms, $y$ is exactly the union of all $y_i$
+and $x$, $y$, and all $z_i$ are disjoint lists of variables. $y$ is called *frontier*. $B$ is called body and the $H_i$ are called heads.
+We call a rule *determinstic* if $k = 1$ so if the head is merely a conjunction.
+
+To represent this formal definition in Lean, we use a structure with a `FunctionFreeConjunction` for the body and a list of `FunctionFreeConjunction`s for the disjunction in the head. For bookkeeping each rule also gets an id. That's it!
+The frontier variables can simply be defined as the variables occurring both in body and head and the existential variables can be indentified as the variables that occur only in the head, without the need for explicit quantification.
+-/
+
+/-- The definition of a `Rule` as discussed above. -/
+structure Rule (sig : Signature) [DecidableEq sig.P] [DecidableEq sig.C] [DecidableEq sig.V] where
+  id : Nat
+  body : FunctionFreeConjunction sig
+  head : List (FunctionFreeConjunction sig)
+deriving DecidableEq
+
 namespace Rule
 
-  def frontier_for_head (r : Rule sig) (i : Fin r.head.length) : List sig.V :=
-    r.body.vars.filter (fun v => v ∈ r.head[i.val].vars)
+variable {sig : Signature} [DecidableEq sig.P] [DecidableEq sig.C] [DecidableEq sig.V]
 
-  def frontier (r : Rule sig) : List sig.V :=
-    r.body.vars.filter (fun v => r.head.any (fun h => v ∈ h.vars))
+/-- This function returns the frontier variables that occur in a given head disjunct. This is a sublist of all the frontier variables. -/
+def frontier_for_head (r : Rule sig) (i : Fin r.head.length) : List sig.V :=
+  r.body.vars.filter (fun v => v ∈ r.head[i.val].vars)
 
-  theorem mem_frontier_iff_mem_frontier_for_head {r : Rule sig} {v : sig.V} :
-      v ∈ r.frontier ↔ ∃ i, v ∈ r.frontier_for_head i := by
-    unfold frontier frontier_for_head; simp only [List.mem_filter, List.any_eq_true, decide_eq_true_iff]
-    constructor
-    . rintro ⟨mem_body, ⟨h, h_mem, mem_h⟩⟩
-      rw [List.mem_iff_getElem] at h_mem
-      rcases h_mem with ⟨i, lt, h_mem⟩
-      exists ⟨i, lt⟩
-      constructor
-      . exact mem_body
-      . rw [h_mem]; exact mem_h
-    . rintro ⟨⟨i, lt⟩, mem_body, mem_h⟩
-      constructor
-      . exact mem_body
-      . exists r.head[i]; constructor; apply List.getElem_mem; exact mem_h
+/-- This returns all the `frontier` variables of the rule, i.e. the variables that occur in both body and some head. -/
+def frontier (r : Rule sig) : List sig.V :=
+  r.body.vars.filter (fun v => r.head.any (fun h => v ∈ h.vars))
 
-  theorem mem_frontier_for_head_of_mem_frontier_of_mem_head_terms {r : Rule sig} {v : sig.V} {i : Fin r.head.length} :
-      v ∈ r.frontier -> VarOrConst.var v ∈ r.head[i.val].terms -> v ∈ r.frontier_for_head i := by
-    unfold frontier frontier_for_head
-    simp only [List.mem_filter, List.any_eq_true, decide_eq_true_iff]
-    rintro ⟨mem_body, _⟩ mem_head_terms
+/-- The `pure_body_vars` are the variables from the body that are not in the `frontier`. -/
+def pure_body_vars (r : Rule sig) : List sig.V := r.body.vars.filter (fun x => x ∉ r.frontier)
+
+/-- We call a rule `isDatalog` if it does not contain existential variables, i.e. if all head variables occur in the body. -/
+def isDatalog (r : Rule sig) : Bool :=
+  r.head.all (fun h => h.vars.all (fun v => v ∈ r.body.vars))
+
+/-- We call a rule `isDeterministic` if it has exactly one head disjunct. -/
+def isDeterministic (r : Rule sig) : Bool := r.head.length = 1
+
+/-- The predicate symbols of a rule are just the predicate symbols from the body and all heads. -/
+def predicates (r : Rule sig) : List sig.P := r.body.predicates ++ (r.head.flatMap FunctionFreeConjunction.predicates)
+
+/-- The constants of a rule are just the constants from the body and all heads. -/
+def constants (r : Rule sig) : List sig.C := r.body.consts ++ r.head.flatMap (fun conj => conj.consts)
+
+/-- Sometimes we require only the constants from the heads and therefore we define them here. -/
+def head_constants (r : Rule sig) : List sig.C := r.head.flatMap (fun conj => conj.consts)
+
+/-- The existential variables for a given head are simply the variables from the head that are not in the frontier. -/
+def existential_vars_for_head_disjunct (r : Rule sig) (i : Nat) (lt : i < r.head.length) : List sig.V :=
+  r.head[i].vars.filter (fun v => v ∉ r.frontier)
+
+/-- The Skolem function symbols of a rule are all `SkolemFS` with the rule id, all possible head indices and the respective existential variables. -/
+def skolem_functions (r : Rule sig) : List (SkolemFS sig) := r.head.zipIdx.flatMap (fun (head, i) =>
+  (head.vars.filter (fun v => v ∉ r.frontier)).map (fun v => { ruleId := r.id, disjunctIndex := i, var := v, arity := r.frontier.length })
+)
+
+/-- A variable is a frontier variable if and only if it is a frontier variable in some head disjunct. -/
+theorem mem_frontier_iff_mem_frontier_for_head {r : Rule sig} {v : sig.V} :
+    v ∈ r.frontier ↔ ∃ i, v ∈ r.frontier_for_head i := by
+  unfold frontier frontier_for_head; simp only [List.mem_filter, List.any_eq_true, decide_eq_true_iff]
+  constructor
+  . rintro ⟨mem_body, ⟨h, h_mem, mem_h⟩⟩
+    rw [List.mem_iff_getElem] at h_mem
+    rcases h_mem with ⟨i, lt, h_mem⟩
+    exists ⟨i, lt⟩
     constructor
     . exact mem_body
-    . unfold FunctionFreeConjunction.terms at mem_head_terms
-      rw [List.mem_flatMap] at mem_head_terms
-      rcases mem_head_terms with ⟨a, a_mem, mem_a⟩
-      rw [FunctionFreeConjunction.mem_vars]; exists a
+    . rw [h_mem]; exact mem_h
+  . rintro ⟨⟨i, lt⟩, mem_body, mem_h⟩
+    constructor
+    . exact mem_body
+    . exists r.head[i]; constructor; apply List.getElem_mem; exact mem_h
 
-  theorem frontier_subset_vars_body {r : Rule sig} : r.frontier ⊆ r.body.vars := by
-    intro v v_mem
-    unfold Rule.frontier at v_mem; rw [List.mem_filter] at v_mem
-    exact v_mem.left
+/-- A variable is in the frontier of a head if it is in the frontier of the rule and occurs as a term in the given head. -/
+theorem mem_frontier_for_head_of_mem_frontier_of_mem_head_terms {r : Rule sig} {v : sig.V} {i : Fin r.head.length} :
+    v ∈ r.frontier -> VarOrConst.var v ∈ r.head[i.val].terms -> v ∈ r.frontier_for_head i := by
+  unfold frontier frontier_for_head
+  simp only [List.mem_filter, List.any_eq_true, decide_eq_true_iff]
+  rintro ⟨mem_body, _⟩ mem_head_terms
+  constructor
+  . exact mem_body
+  . unfold FunctionFreeConjunction.terms at mem_head_terms
+    rw [List.mem_flatMap] at mem_head_terms
+    rcases mem_head_terms with ⟨a, a_mem, mem_a⟩
+    rw [FunctionFreeConjunction.mem_vars]; exists a
 
-  theorem frontier_for_head_subset_vars_head {r : Rule sig} {i : Nat} {lt : i < r.head.length} : r.frontier_for_head ⟨i, lt⟩ ⊆ r.head[i].vars := by
-    intro v v_mem
-    unfold Rule.frontier_for_head at v_mem; rw [List.mem_filter] at v_mem
-    rw [decide_eq_true_iff] at v_mem
-    exact v_mem.right
+/-- All frontier variables occur in the body. -/
+theorem frontier_subset_vars_body {r : Rule sig} : r.frontier ⊆ r.body.vars := by
+  intro v v_mem
+  unfold Rule.frontier at v_mem; rw [List.mem_filter] at v_mem
+  exact v_mem.left
 
-  def pure_body_vars (r : Rule sig) : List sig.V := r.body.vars.filter (fun x => x ∉ r.frontier)
+/-- The frontier variables in a given head occur in the list of variables for the same head. -/
+theorem frontier_for_head_subset_vars_head {r : Rule sig} {i : Nat} {lt : i < r.head.length} : r.frontier_for_head ⟨i, lt⟩ ⊆ r.head[i].vars := by
+  intro v v_mem
+  unfold Rule.frontier_for_head at v_mem; rw [List.mem_filter] at v_mem
+  rw [decide_eq_true_iff] at v_mem
+  exact v_mem.right
 
-  def isDatalog (r : Rule sig) : Bool :=
-    r.head.all (fun h => h.vars.all (fun v => v ∈ r.body.vars))
-
-  def isDeterministic (r : Rule sig) : Bool := r.head.length = 1
-
-  def predicates (r : Rule sig) : List sig.P := r.body.predicates ++ (r.head.flatMap FunctionFreeConjunction.predicates)
-
-  def constants (r : Rule sig) : List sig.C := r.body.consts ++ r.head.flatMap (fun conj => conj.consts)
-
-  def head_constants (r : Rule sig) : List sig.C := r.head.flatMap (fun conj => conj.consts)
-
-  theorem head_constants_subset_constants (r : Rule sig) : r.head_constants ⊆ r.constants := by apply List.subset_append_right
-
-  def skolem_functions (r : Rule sig) : List (SkolemFS sig) := r.head.zipIdx.flatMap (fun (head, i) =>
-    (head.vars.filter (fun v => !(v ∈ r.frontier))).map (fun v => { ruleId := r.id, disjunctIndex := i, var := v, arity := r.frontier.length })
-  )
-
-  def existential_vars_for_head_disjunct (r : Rule sig) (i : Nat) (lt : i < r.head.length) : List sig.V :=
-    r.head[i].vars.filter (fun v => v ∉ r.frontier)
+/-- The head constants of the rule are also constants of the whole rule. -/
+theorem head_constants_subset_constants (r : Rule sig) : r.head_constants ⊆ r.constants := by apply List.subset_append_right
 
 end Rule
 
+end Rule
+
+section RuleSetAndRuleList
+
+/-!
+## RuleSet and RuleList
+-/
+
+/-- A `RuleSet` is a `Set (Rule sig)` where rules are uniquely identified by their id. -/
+structure RuleSet (sig : Signature) [DecidableEq sig.P] [DecidableEq sig.C] [DecidableEq sig.V] where
+  rules : Set (Rule sig)
+  id_unique : ∀ r1 r2, r1 ∈ rules ∧ r2 ∈ rules ∧ r1.id = r2.id -> r1 = r2
+
+/-- A `RuleList` is a `List (Rule sig)` where rules are uniquely identified by their id. -/
+structure RuleList (sig : Signature) [DecidableEq sig.P] [DecidableEq sig.C] [DecidableEq sig.V] where
+  rules : List (Rule sig)
+  id_unique : ∀ r1 r2, r1 ∈ rules ∧ r2 ∈ rules ∧ r1.id = r2.id -> r1 = r2
+
 namespace RuleSet
 
-  def isDeterministic (rs : RuleSet sig) : Prop := ∀ (r : Rule sig), r ∈ rs.rules -> r.isDeterministic
+/-!
+### RuleSet
+-/
 
-  def predicates (rs : RuleSet sig) : Set sig.P := fun p => ∃ r, r ∈ rs.rules ∧ p ∈ r.predicates
+variable {sig : Signature} [DecidableEq sig.P] [DecidableEq sig.C] [DecidableEq sig.V]
 
-  theorem predicates_finite_of_finite (rs : RuleSet sig) : rs.rules.finite -> rs.predicates.finite := by
-    intro finite
-    rcases finite with ⟨l, nodup, eq⟩
-    exists (l.flatMap Rule.predicates).eraseDupsKeepRight
-    constructor
-    . apply List.nodup_eraseDupsKeepRight
-    . intro p
-      rw [List.mem_eraseDupsKeepRight]
-      unfold predicates
-      simp only [List.mem_flatMap]
-      constructor <;> (intro h; rcases h with ⟨r, h⟩; exists r)
-      . rw [← eq]; assumption
-      . rw [eq]; assumption
+/-- A `RuleSet` is is deterministic if each rule is. -/
+def isDeterministic (rs : RuleSet sig) : Prop := ∀ (r : Rule sig), r ∈ rs.rules -> r.isDeterministic
 
-  def constants (rs : RuleSet sig) : Set sig.C := fun c => ∃ r, r ∈ rs.rules ∧ c ∈ r.constants
+/-- The predicate symbols of a `RuleSet` are the predicate symbols from all rules. -/
+def predicates (rs : RuleSet sig) : Set sig.P := fun p => ∃ r, r ∈ rs.rules ∧ p ∈ r.predicates
 
-  theorem constants_finite_of_finite (rs : RuleSet sig) : rs.rules.finite -> rs.constants.finite := by
-    intro finite
-    rcases finite with ⟨l, nodup, eq⟩
-    exists (l.flatMap Rule.constants).eraseDupsKeepRight
-    constructor
-    . apply List.nodup_eraseDupsKeepRight
-    . intro c
-      rw [List.mem_eraseDupsKeepRight]
-      unfold constants
-      simp only [List.mem_flatMap]
-      constructor <;> (intro h; rcases h with ⟨r, h⟩; exists r)
-      . rw [← eq]; assumption
-      . rw [eq]; assumption
+/-- The constants of a `RuleSet` are the constants from all rules. -/
+def constants (rs : RuleSet sig) : Set sig.C := fun c => ∃ r, r ∈ rs.rules ∧ c ∈ r.constants
 
-  def head_constants (rs : RuleSet sig) : Set sig.C := fun c => ∃ r, r ∈ rs.rules ∧ c ∈ r.head_constants
+/-- The head constants of a `RuleSet` are the head constants from all rules. -/
+def head_constants (rs : RuleSet sig) : Set sig.C := fun c => ∃ r, r ∈ rs.rules ∧ c ∈ r.head_constants
 
-  theorem head_constants_finite_of_finite (rs : RuleSet sig) : rs.rules.finite -> rs.head_constants.finite := by
-    intro finite
-    rcases finite with ⟨l, nodup, eq⟩
-    exists (l.flatMap Rule.head_constants).eraseDupsKeepRight
-    constructor
-    . apply List.nodup_eraseDupsKeepRight
-    . intro c
-      rw [List.mem_eraseDupsKeepRight]
-      unfold head_constants
-      simp only [List.mem_flatMap]
-      constructor <;> (intro h; rcases h with ⟨r, h⟩; exists r)
-      . rw [← eq]; assumption
-      . rw [eq]; assumption
+/-- The Skolem function symbols of a `RuleSet` are the Skolem function symbols from all rules. -/
+def skolem_functions (rs : RuleSet sig) : Set (SkolemFS sig) := fun f => ∃ r, r ∈ rs.rules ∧ f ∈ r.skolem_functions
 
-  theorem head_constants_subset_constants (rs : RuleSet sig) : rs.head_constants ⊆ rs.constants := by
-    intro c c_mem
-    rcases c_mem with ⟨r, r_mem, c_mem⟩
-    exists r
-    constructor
-    . exact r_mem
-    . apply Rule.head_constants_subset_constants; exact c_mem
+/-- If the `RuleSet` is finite, so are the `predicates`. -/
+theorem predicates_finite_of_finite (rs : RuleSet sig) : rs.rules.finite -> rs.predicates.finite := by
+  intro finite
+  rcases finite with ⟨l, nodup, eq⟩
+  exists (l.flatMap Rule.predicates).eraseDupsKeepRight
+  constructor
+  . apply List.nodup_eraseDupsKeepRight
+  . intro p
+    rw [List.mem_eraseDupsKeepRight]
+    unfold predicates
+    simp only [List.mem_flatMap]
+    constructor <;> (intro h; rcases h with ⟨r, h⟩; exists r)
+    . rw [← eq]; assumption
+    . rw [eq]; assumption
 
-  def skolem_functions (rs : RuleSet sig) : Set (SkolemFS sig) := fun f => ∃ r, r ∈ rs.rules ∧ f ∈ r.skolem_functions
+/-- If the `RuleSet` is finite, so are the `constants`. -/
+theorem constants_finite_of_finite (rs : RuleSet sig) : rs.rules.finite -> rs.constants.finite := by
+  intro finite
+  rcases finite with ⟨l, nodup, eq⟩
+  exists (l.flatMap Rule.constants).eraseDupsKeepRight
+  constructor
+  . apply List.nodup_eraseDupsKeepRight
+  . intro c
+    rw [List.mem_eraseDupsKeepRight]
+    unfold constants
+    simp only [List.mem_flatMap]
+    constructor <;> (intro h; rcases h with ⟨r, h⟩; exists r)
+    . rw [← eq]; assumption
+    . rw [eq]; assumption
 
-  theorem skolem_functions_finite_of_finite (rs : RuleSet sig) : rs.rules.finite -> rs.skolem_functions.finite := by
-    intro finite
-    rcases finite with ⟨l, nodup, eq⟩
-    exists (l.flatMap Rule.skolem_functions).eraseDupsKeepRight
-    constructor
-    . apply List.nodup_eraseDupsKeepRight
-    . intro c
-      rw [List.mem_eraseDupsKeepRight]
-      unfold skolem_functions
-      simp only [List.mem_flatMap]
-      constructor <;> (intro h; rcases h with ⟨r, h⟩; exists r)
-      . rw [← eq]; assumption
-      . rw [eq]; assumption
+/-- If the `RuleSet` is finite, so are the `head_constants`. -/
+theorem head_constants_finite_of_finite (rs : RuleSet sig) : rs.rules.finite -> rs.head_constants.finite := by
+  intro finite
+  rcases finite with ⟨l, nodup, eq⟩
+  exists (l.flatMap Rule.head_constants).eraseDupsKeepRight
+  constructor
+  . apply List.nodup_eraseDupsKeepRight
+  . intro c
+    rw [List.mem_eraseDupsKeepRight]
+    unfold head_constants
+    simp only [List.mem_flatMap]
+    constructor <;> (intro h; rcases h with ⟨r, h⟩; exists r)
+    . rw [← eq]; assumption
+    . rw [eq]; assumption
+
+/-- If the `RuleSet` is finite, so are the `skolem_functions`. -/
+theorem skolem_functions_finite_of_finite (rs : RuleSet sig) : rs.rules.finite -> rs.skolem_functions.finite := by
+  intro finite
+  rcases finite with ⟨l, nodup, eq⟩
+  exists (l.flatMap Rule.skolem_functions).eraseDupsKeepRight
+  constructor
+  . apply List.nodup_eraseDupsKeepRight
+  . intro c
+    rw [List.mem_eraseDupsKeepRight]
+    unfold skolem_functions
+    simp only [List.mem_flatMap]
+    constructor <;> (intro h; rcases h with ⟨r, h⟩; exists r)
+    . rw [← eq]; assumption
+    . rw [eq]; assumption
+
+/-- The `head_constants` of a `RuleSet` are a subset of the `constants`. -/
+theorem head_constants_subset_constants (rs : RuleSet sig) : rs.head_constants ⊆ rs.constants := by
+  intro c c_mem
+  rcases c_mem with ⟨r, r_mem, c_mem⟩
+  exists r
+  constructor
+  . exact r_mem
+  . apply Rule.head_constants_subset_constants; exact c_mem
 
 end RuleSet
 
 namespace RuleList
 
-  def get_by_id (rl : RuleList sig) (id : Nat) (id_mem : ∃ r ∈ rl.rules, r.id = id) : Rule sig :=
-    (rl.rules.find? (fun r => r.id = id)).get (by simp [id_mem])
+/-!
+### RuleList
+-/
 
-  theorem get_by_id_mem (rl : RuleList sig) (id : Nat) (id_mem : ∃ r ∈ rl.rules, r.id = id) : rl.get_by_id id id_mem ∈ rl.rules := by unfold get_by_id; apply List.get_find?_mem
+variable {sig : Signature} [DecidableEq sig.P] [DecidableEq sig.C] [DecidableEq sig.V]
 
-  theorem get_by_id_self (rl : RuleList sig) (r : Rule sig) (mem : r ∈ rl.rules) : rl.get_by_id r.id (by exists r) = r := by
-    apply rl.id_unique
-    constructor
-    . apply List.get_find?_mem
-    constructor
-    . exact mem
-    . unfold get_by_id
-      have eq : rl.rules.find? (fun r' => r'.id = r.id) = some ((rl.rules.find? (fun r' => r'.id = r.id)).get (by rw [List.find?_isSome]; exists r; constructor; exact mem; simp)) := by simp
-      apply of_decide_eq_true
-      apply List.find?_some eq
+/-- In a `RuleList`, we can obtain a rule based on its id. -/
+def get_by_id (rl : RuleList sig) (id : Nat) (id_mem : ∃ r ∈ rl.rules, r.id = id) : Rule sig :=
+  (rl.rules.find? (fun r => r.id = id)).get (by simp [id_mem])
+
+/-- A rule that we get by id is in the `RuleList`. -/
+theorem get_by_id_mem (rl : RuleList sig) (id : Nat) (id_mem : ∃ r ∈ rl.rules, r.id = id) : rl.get_by_id id id_mem ∈ rl.rules := by unfold get_by_id; apply List.get_find?_mem
+
+/-- A rule that we get by id is indeed the rule that the id belongs to. -/
+theorem get_by_id_self (rl : RuleList sig) (r : Rule sig) (mem : r ∈ rl.rules) : rl.get_by_id r.id (by exists r) = r := by
+  apply rl.id_unique
+  constructor
+  . apply List.get_find?_mem
+  constructor
+  . exact mem
+  . unfold get_by_id
+    have eq : rl.rules.find? (fun r' => r'.id = r.id) = some ((rl.rules.find? (fun r' => r'.id = r.id)).get (by rw [List.find?_isSome]; exists r; constructor; exact mem; simp)) := by simp
+    apply of_decide_eq_true
+    apply List.find?_some eq
 
 end RuleList
 
+end RuleSetAndRuleList
 
-namespace KnowledgeBase
+section FactAndFunctionFreeFact
 
-  def isDeterministic (kb : KnowledgeBase sig) : Prop := kb.rules.isDeterministic
+/-!
+## Facts and FunctionFreeFacts
+-/
 
-end KnowledgeBase
+/-- A `Fact` is a `GeneralizedAtom` with `GroundTerm`s. -/
+abbrev Fact (sig : Signature) [DecidableEq sig.P] [DecidableEq sig.C] [DecidableEq sig.V] := GeneralizedAtom sig (GroundTerm sig)
+
+/-- A `FunctionFreeFact` is a `GeneralizedAtom` with constants. -/
+abbrev FunctionFreeFact (sig : Signature) [DecidableEq sig.P] := GeneralizedAtom sig sig.C
 
 namespace Fact
 
-  def constants (f : Fact sig) : List sig.C := f.terms.flatMap GroundTerm.constants
+variable {sig : Signature} [DecidableEq sig.P] [DecidableEq sig.C] [DecidableEq sig.V]
 
-  def function_symbols (f : Fact sig) : List (SkolemFS sig) := f.terms.flatMap GroundTerm.functions
+/-- The `constants` of a `Fact` are the constants of all terms. -/
+def constants (f : Fact sig) : List sig.C := f.terms.flatMap GroundTerm.constants
 
-  def isFunctionFree (f : Fact sig) : Prop := ∀ t, t ∈ f.terms -> ∃ c, t = GroundTerm.const c
+/-- The `function_symbols` of a `Fact` are the function symbols of all terms. -/
+def function_symbols (f : Fact sig) : List (SkolemFS sig) := f.terms.flatMap GroundTerm.functions
 
-  def toFunctionFreeFact (f : Fact sig) (isFunctionFree : f.isFunctionFree) : FunctionFreeFact sig := {
-    predicate := f.predicate
-    terms := f.terms.attach.map (fun t => t.val.toConst (isFunctionFree t.val t.property))
-    arity_ok := by rw [List.length_map, List.length_attach, f.arity_ok]
-  }
+/-- A `Fact` is function free, if each term is a constant. -/
+def isFunctionFree (f : Fact sig) : Prop := ∀ t, t ∈ f.terms -> ∃ c, t = GroundTerm.const c
+
+/-- If a `Fact` `isFunctionFree`, then we can convert it to a `FunctionFreeFact`. -/
+def toFunctionFreeFact (f : Fact sig) (isFunctionFree : f.isFunctionFree) : FunctionFreeFact sig := {
+  predicate := f.predicate
+  terms := f.terms.attach.map (fun t => t.val.toConst (isFunctionFree t.val t.property))
+  arity_ok := by rw [List.length_map, List.length_attach, f.arity_ok]
+}
 
 end Fact
 
 namespace FunctionFreeFact
 
-  def toFact (f : FunctionFreeFact sig) : Fact sig := {
-    predicate := f.predicate,
-    terms := f.terms.map GroundTerm.const,
-    arity_ok := by rw [List.length_map, f.arity_ok]
-  }
+variable {sig : Signature} [DecidableEq sig.P] [DecidableEq sig.C] [DecidableEq sig.V]
 
-  theorem toFact_isFunctionFree (f : FunctionFreeFact sig) : f.toFact.isFunctionFree := by
-    intro t t_mem
-    unfold toFact at t_mem
-    simp at t_mem
-    rcases t_mem with ⟨c, _, t_eq⟩
-    exists c
-    rw [t_eq]
+/-- A `FunctionFreeFact` can always be converted to a `Fact`. -/
+def toFact (f : FunctionFreeFact sig) : Fact sig := {
+  predicate := f.predicate,
+  terms := f.terms.map GroundTerm.const,
+  arity_ok := by rw [List.length_map, f.arity_ok]
+}
 
-  theorem toFunctionFreeFact_after_toFact_is_id (f : FunctionFreeFact sig) : f.toFact.toFunctionFreeFact (f.toFact_isFunctionFree) = f := by
-    unfold toFact
-    unfold Fact.toFunctionFreeFact
-    simp only
-    rw [GeneralizedAtom.mk.injEq]
-    constructor
-    . simp
-    . rw [List.map_attach_eq_pmap, List.pmap_map]
-      simp [GroundTerm.toConst, GroundTerm.const]
+/-- A `Fact` obtained from a `FunctionFreeFact` `isFunctionFree`. -/
+theorem toFact_isFunctionFree (f : FunctionFreeFact sig) : f.toFact.isFunctionFree := by
+  intro t t_mem
+  unfold toFact at t_mem
+  simp at t_mem
+  rcases t_mem with ⟨c, _, t_eq⟩
+  exists c
+  rw [t_eq]
+
+/-- Converting a `FunctionFreeFact` to a `Fact` and back yields the initial `FunctionFreeFact`. -/
+theorem toFunctionFreeFact_after_toFact_is_id (f : FunctionFreeFact sig) : f.toFact.toFunctionFreeFact (f.toFact_isFunctionFree) = f := by
+  unfold toFact
+  unfold Fact.toFunctionFreeFact
+  simp only
+  rw [GeneralizedAtom.mk.injEq]
+  constructor
+  . simp
+  . rw [List.map_attach_eq_pmap, List.pmap_map]
+    simp [GroundTerm.toConst, GroundTerm.const]
 
 end FunctionFreeFact
 
-theorem Fact.toFact_after_toFunctionFreeFact_is_id (f : Fact sig) (isFunctionFree : f.isFunctionFree) : (f.toFunctionFreeFact isFunctionFree).toFact = f := by
+namespace Fact
+
+variable {sig : Signature} [DecidableEq sig.P] [DecidableEq sig.C] [DecidableEq sig.V]
+
+/-- Converting a `Fact` to a `FunctionFreeFact` and back yields the initial `Fact`. -/
+theorem toFact_after_toFunctionFreeFact_is_id (f : Fact sig) (isFunctionFree : f.isFunctionFree) : (f.toFunctionFreeFact isFunctionFree).toFact = f := by
   unfold toFunctionFreeFact
   unfold FunctionFreeFact.toFact
   simp
@@ -353,253 +476,322 @@ theorem Fact.toFact_after_toFunctionFreeFact_is_id (f : Fact sig) (isFunctionFre
     unfold GroundTerm.toConst
     simp
 
+end Fact
+
+end FactAndFunctionFreeFact
+
+section FactSet
+
+/-!
+## FactSet
+-/
+
+/-- A `FactSet` is plainly a `Set` of `Fact`s. -/
+abbrev FactSet (sig : Signature) [DecidableEq sig.P] [DecidableEq sig.C] [DecidableEq sig.V] := Set (Fact sig)
+
 namespace FactSet
 
-  def predicates (fs : FactSet sig) : Set sig.P := fun p => ∃ f, f ∈ fs ∧ f.predicate = p
+variable {sig : Signature} [DecidableEq sig.P] [DecidableEq sig.C] [DecidableEq sig.V]
 
-  def terms (fs : FactSet sig) : Set (GroundTerm sig) := fun t => ∃ f, f ∈ fs ∧ t ∈ f.terms
+/-- The predicate symbols of a `FactSet` are the predicate symbols from all facts. -/
+def predicates (fs : FactSet sig) : Set sig.P := fun p => ∃ f, f ∈ fs ∧ f.predicate = p
 
-  def constants (fs : FactSet sig) : Set sig.C := fun c => ∃ f, f ∈ fs ∧ c ∈ f.constants
+/-- The terms of a `FactSet` are the terms from all facts. -/
+def terms (fs : FactSet sig) : Set (GroundTerm sig) := fun t => ∃ f, f ∈ fs ∧ t ∈ f.terms
 
-  def function_symbols (fs : FactSet sig) : Set (SkolemFS sig) := fun func => ∃ f, f ∈ fs ∧ func ∈ f.function_symbols
+/-- The constants of a `FactSet` are the constants from all facts. -/
+def constants (fs : FactSet sig) : Set sig.C := fun c => ∃ f, f ∈ fs ∧ c ∈ f.constants
 
-  def isFunctionFree (fs : FactSet sig) : Prop := ∀ f, f ∈ fs -> f.isFunctionFree
+/-- The function symbols of a `FactSet` are the function symbols from all facts. -/
+def function_symbols (fs : FactSet sig) : Set (SkolemFS sig) := fun func => ∃ f, f ∈ fs ∧ func ∈ f.function_symbols
 
-  theorem mem_terms_toSet {l : List (Fact sig)} : ∀ t, t ∈ FactSet.terms (l.toSet) ↔ t ∈ l.flatMap GeneralizedAtom.terms := by
-    intro t; rw [List.mem_flatMap]
-    constructor <;> (rintro ⟨f, f_mem, t_mem⟩; exists f)
+/-- A `FactSet` is function free if all of its facts are. -/
+def isFunctionFree (fs : FactSet sig) : Prop := ∀ f, f ∈ fs -> f.isFunctionFree
 
-  theorem terms_subset_of_subset {fs1 fs2 : FactSet sig} : fs1 ⊆ fs2 -> fs1.terms ⊆ fs2.terms := by
-    rintro sub t ⟨f, f_mem, t_mem⟩; exists f; exact ⟨sub _ f_mem, t_mem⟩
+/-- When converting a list to a `FactSet`, the terms remain the same. -/
+theorem mem_terms_toSet {l : List (Fact sig)} : ∀ t, t ∈ FactSet.terms (l.toSet) ↔ t ∈ l.flatMap GeneralizedAtom.terms := by
+  intro t; rw [List.mem_flatMap]
+  constructor <;> (rintro ⟨f, f_mem, t_mem⟩; exists f)
 
-  theorem terms_union {fs1 fs2 : FactSet sig} : (fs1 ∪ fs2).terms = fs1.terms ∪ fs2.terms := by
-    apply Set.ext
-    intro t; constructor
-    . rintro ⟨f, f_mem, t_mem⟩; cases f_mem with | inl f_mem => apply Or.inl; exists f | inr f_mem => apply Or.inr; exists f
-    . intro t_mem; cases t_mem with
-      | inl t_mem => rcases t_mem with ⟨f, f_mem, t_mem⟩; exists f; simp only [t_mem, and_true]; exact Or.inl f_mem
-      | inr t_mem => rcases t_mem with ⟨f, f_mem, t_mem⟩; exists f; simp only [t_mem, and_true]; exact Or.inr f_mem
+/-- The a `FactSet` is a subset of another, then their terms share this subset relation. -/
+theorem terms_subset_of_subset {fs1 fs2 : FactSet sig} : fs1 ⊆ fs2 -> fs1.terms ⊆ fs2.terms := by
+  rintro sub t ⟨f, f_mem, t_mem⟩; exists f; exact ⟨sub _ f_mem, t_mem⟩
 
-  theorem terms_finite_of_finite (fs : FactSet sig) (finite : fs.finite) : fs.terms.finite := by
-    rcases finite with ⟨l, nodup, finite⟩
-    exists (l.map GeneralizedAtom.terms).flatten.eraseDupsKeepRight
+/-- The terms of the union of two `FactSet`s are the union of the terms of both sets. -/
+theorem terms_union {fs1 fs2 : FactSet sig} : (fs1 ∪ fs2).terms = fs1.terms ∪ fs2.terms := by
+  apply Set.ext
+  intro t; constructor
+  . rintro ⟨f, f_mem, t_mem⟩; cases f_mem with | inl f_mem => apply Or.inl; exists f | inr f_mem => apply Or.inr; exists f
+  . intro t_mem; cases t_mem with
+    | inl t_mem => rcases t_mem with ⟨f, f_mem, t_mem⟩; exists f; simp only [t_mem, and_true]; exact Or.inl f_mem
+    | inr t_mem => rcases t_mem with ⟨f, f_mem, t_mem⟩; exists f; simp only [t_mem, and_true]; exact Or.inr f_mem
+
+/-- If a `FactSet` is finite, so are its terms. -/
+theorem terms_finite_of_finite (fs : FactSet sig) (finite : fs.finite) : fs.terms.finite := by
+  rcases finite with ⟨l, nodup, finite⟩
+  exists (l.map GeneralizedAtom.terms).flatten.eraseDupsKeepRight
+  constructor
+  . apply List.nodup_eraseDupsKeepRight
+  . intro e
     constructor
-    . apply List.nodup_eraseDupsKeepRight
-    . intro e
+    . intro in_l
+      unfold FactSet.terms
+      simp [List.mem_eraseDupsKeepRight, List.mem_flatten] at in_l
+      rcases in_l with ⟨terms, ex_f, e_in_terms⟩
+      rcases ex_f with ⟨f, f_in_l, terms_eq⟩
+      exists f
       constructor
-      . intro in_l
-        unfold FactSet.terms
-        simp [List.mem_eraseDupsKeepRight, List.mem_flatten] at in_l
-        rcases in_l with ⟨terms, ex_f, e_in_terms⟩
-        rcases ex_f with ⟨f, f_in_l, terms_eq⟩
-        exists f
+      . rw [← finite]; exact f_in_l
+      . rw [terms_eq]; exact e_in_terms
+    . intro in_fs
+      unfold FactSet.terms at in_fs
+      simp [List.mem_eraseDupsKeepRight, List.mem_flatten]
+      rcases in_fs with ⟨f, f_in_fs, e_in_f⟩
+      exists f.terms
+      constructor
+      . exists f
         constructor
-        . rw [← finite]; exact f_in_l
-        . rw [terms_eq]; exact e_in_terms
-      . intro in_fs
-        unfold FactSet.terms at in_fs
-        simp [List.mem_eraseDupsKeepRight, List.mem_flatten]
-        rcases in_fs with ⟨f, f_in_fs, e_in_f⟩
-        exists f.terms
-        constructor
-        . exists f
-          constructor
-          . rw [finite]; exact f_in_fs
-          . rfl
-        . exact e_in_f
+        . rw [finite]; exact f_in_fs
+        . rfl
+      . exact e_in_f
 
-  theorem mem_constants_toSet {l : List (Fact sig)} : ∀ c, c ∈ FactSet.constants (l.toSet) ↔ c ∈ l.flatMap Fact.constants := by
-    intro t; rw [List.mem_flatMap]
-    constructor <;> (rintro ⟨f, f_mem, t_mem⟩; exists f)
+/-- When converting a list to a `FactSet`, the constants remain the same. -/
+theorem mem_constants_toSet {l : List (Fact sig)} : ∀ c, c ∈ FactSet.constants (l.toSet) ↔ c ∈ l.flatMap Fact.constants := by
+  intro t; rw [List.mem_flatMap]
+  constructor <;> (rintro ⟨f, f_mem, t_mem⟩; exists f)
 
-  theorem constants_union {fs1 fs2 : FactSet sig} : (fs1 ∪ fs2).constants = fs1.constants ∪ fs2.constants := by
-    -- NOTE: same proof as terms_union
-    apply Set.ext
-    intro t; constructor
-    . rintro ⟨f, f_mem, t_mem⟩; cases f_mem with | inl f_mem => apply Or.inl; exists f | inr f_mem => apply Or.inr; exists f
-    . intro t_mem; cases t_mem with
-      | inl t_mem => rcases t_mem with ⟨f, f_mem, t_mem⟩; exists f; simp only [t_mem, and_true]; exact Or.inl f_mem
-      | inr t_mem => rcases t_mem with ⟨f, f_mem, t_mem⟩; exists f; simp only [t_mem, and_true]; exact Or.inr f_mem
+/-- The constants of the union of two `FactSet`s are the union of the constants of both sets. -/
+theorem constants_union {fs1 fs2 : FactSet sig} : (fs1 ∪ fs2).constants = fs1.constants ∪ fs2.constants := by
+  -- NOTE: same proof as terms_union
+  apply Set.ext
+  intro t; constructor
+  . rintro ⟨f, f_mem, t_mem⟩; cases f_mem with | inl f_mem => apply Or.inl; exists f | inr f_mem => apply Or.inr; exists f
+  . intro t_mem; cases t_mem with
+    | inl t_mem => rcases t_mem with ⟨f, f_mem, t_mem⟩; exists f; simp only [t_mem, and_true]; exact Or.inl f_mem
+    | inr t_mem => rcases t_mem with ⟨f, f_mem, t_mem⟩; exists f; simp only [t_mem, and_true]; exact Or.inr f_mem
 
-  theorem constants_finite_of_finite (fs : FactSet sig) (fin : fs.finite) : fs.constants.finite := by
-    rcases fin with ⟨l, _, l_eq⟩
-    exists (l.flatMap Fact.constants).eraseDupsKeepRight
+/-- If a `FactSet` is finite, so are its constants. -/
+theorem constants_finite_of_finite (fs : FactSet sig) (fin : fs.finite) : fs.constants.finite := by
+  rcases fin with ⟨l, _, l_eq⟩
+  exists (l.flatMap Fact.constants).eraseDupsKeepRight
+  constructor
+  . apply List.nodup_eraseDupsKeepRight
+  . intro c
+    rw [List.mem_eraseDupsKeepRight]
+    rw [List.mem_flatMap]
+    unfold constants
     constructor
-    . apply List.nodup_eraseDupsKeepRight
-    . intro c
-      rw [List.mem_eraseDupsKeepRight]
-      rw [List.mem_flatMap]
-      unfold constants
-      constructor
-      . intro h
-        rcases h with ⟨f, f_mem, c_mem⟩
-        rw [l_eq] at f_mem
-        exists f
-      . intro h
-        rcases h with ⟨f, f_mem, c_mem⟩
-        rw [← l_eq] at f_mem
-        exists f
-
-  theorem finite_of_preds_finite_of_terms_finite (fs : FactSet sig) : fs.predicates.finite -> fs.terms.finite -> fs.finite := by
-    intro preds_fin terms_fin
-    rcases preds_fin with ⟨preds, _, preds_eq⟩
-    rcases terms_fin with ⟨terms, _, terms_eq⟩
-
-    let overapproximation : FactSet sig := fun f => f.predicate ∈ fs.predicates ∧ (∀ t, t ∈ f.terms -> t ∈ fs.terms)
-    have overapproximation_fin : overapproximation.finite := by
-      exists (preds.flatMap (fun p =>
-        (all_lists_of_length terms (sig.arity p)).attach.map (fun ⟨ts, mem⟩ =>
-          {
-            predicate := p
-            terms := ts
-            arity_ok := ((mem_all_lists_of_length terms (sig.arity p) ts).mp mem).left
-          }
-        )
-      )).eraseDupsKeepRight
-
-      constructor
-      . apply List.nodup_eraseDupsKeepRight
-      . intro f
-        rw [List.mem_eraseDupsKeepRight]
-        simp only [List.mem_flatMap, List.mem_map, List.mem_attach, true_and, Subtype.exists]
-        constructor
-        . intro h
-          rcases h with ⟨pred, pred_mem, ts, ts_mem, f_eq⟩
-          rw [← f_eq]
-          constructor
-          . rw [preds_eq] at pred_mem
-            exact pred_mem
-          . rw [mem_all_lists_of_length] at ts_mem
-            intro t t_mem
-            rw [← terms_eq]
-            apply ts_mem.right
-            exact t_mem
-        . intro h
-          rcases h with ⟨pred_mem, ts_mem⟩
-          exists f.predicate
-          constructor
-          . rw [preds_eq]; exact pred_mem
-          . exists f.terms
-            exists (by
-              rw [mem_all_lists_of_length]
-              constructor
-              . exact f.arity_ok
-              . intro t t_mem; rw [terms_eq]; apply ts_mem; exact t_mem
-            )
-
-    apply Set.finite_of_subset_finite overapproximation_fin
-    intro f f_mem
-    constructor
-    . exists f
-    . intro t t_mem
+    . intro h
+      rcases h with ⟨f, f_mem, c_mem⟩
+      rw [l_eq] at f_mem
+      exists f
+    . intro h
+      rcases h with ⟨f, f_mem, c_mem⟩
+      rw [← l_eq] at f_mem
       exists f
 
-  theorem list_of_facts_for_list_of_terms {ts : List (GroundTerm sig)} {fs : FactSet sig} (ts_sub : ts.toSet ⊆ fs.terms) :
-      ∃ (l : List (Fact sig)), l.toSet ⊆ fs ∧ ts ⊆ l.flatMap GeneralizedAtom.terms := by
-    induction ts with
-    | nil => exists []; constructor; intro _ mem; simp [List.mem_toSet] at mem; simp
-    | cons t ts ih =>
-      rcases (ts_sub t (by simp [List.mem_toSet])) with ⟨f, f_mem, t_mem⟩
-      rcases ih (by intro _ mem; rw [List.mem_toSet] at mem; apply ts_sub; simp [List.mem_toSet, mem]) with ⟨l, l_sub, ts_sub⟩
-      exists (f :: l); constructor
-      . intro _ mem; rw [List.mem_toSet, List.mem_cons] at mem
-        cases mem with
-        | inl mem => rw [mem]; exact f_mem
-        | inr mem => apply l_sub; rw [List.mem_toSet]; exact mem
-      . intro s; rw [List.mem_cons, List.flatMap_cons, List.mem_append]
-        intro s_mem; cases s_mem with
-        | inl s_mem => apply Or.inl; rw [s_mem]; exact t_mem
-        | inr s_mem => apply Or.inr; apply ts_sub; exact s_mem
+/-- A `FactSet` is finite if both its predicates and terms are. This holds since the fact set must be a subset of all facts that can possibly be constructed using the prediactes and terms available. This overapproximation is easily shown to be finite. -/
+theorem finite_of_preds_finite_of_terms_finite (fs : FactSet sig) : fs.predicates.finite -> fs.terms.finite -> fs.finite := by
+  intro preds_fin terms_fin
+  rcases preds_fin with ⟨preds, _, preds_eq⟩
+  rcases terms_fin with ⟨terms, _, terms_eq⟩
+
+  let overapproximation : FactSet sig := fun f => f.predicate ∈ fs.predicates ∧ (∀ t, t ∈ f.terms -> t ∈ fs.terms)
+  have overapproximation_fin : overapproximation.finite := by
+    exists (preds.flatMap (fun p =>
+      (all_lists_of_length terms (sig.arity p)).attach.map (fun ⟨ts, mem⟩ =>
+        {
+          predicate := p
+          terms := ts
+          arity_ok := ((mem_all_lists_of_length terms (sig.arity p) ts).mp mem).left
+        }
+      )
+    )).eraseDupsKeepRight
+
+    constructor
+    . apply List.nodup_eraseDupsKeepRight
+    . intro f
+      rw [List.mem_eraseDupsKeepRight]
+      simp only [List.mem_flatMap, List.mem_map, List.mem_attach, true_and, Subtype.exists]
+      constructor
+      . intro h
+        rcases h with ⟨pred, pred_mem, ts, ts_mem, f_eq⟩
+        rw [← f_eq]
+        constructor
+        . rw [preds_eq] at pred_mem
+          exact pred_mem
+        . rw [mem_all_lists_of_length] at ts_mem
+          intro t t_mem
+          rw [← terms_eq]
+          apply ts_mem.right
+          exact t_mem
+      . intro h
+        rcases h with ⟨pred_mem, ts_mem⟩
+        exists f.predicate
+        constructor
+        . rw [preds_eq]; exact pred_mem
+        . exists f.terms
+          exists (by
+            rw [mem_all_lists_of_length]
+            constructor
+            . exact f.arity_ok
+            . intro t t_mem; rw [terms_eq]; apply ts_mem; exact t_mem
+          )
+
+  apply Set.finite_of_subset_finite overapproximation_fin
+  intro f f_mem
+  constructor
+  . exists f
+  . intro t t_mem
+    exists f
+
+/-- For a list of terms in a given `FactSet`, we can find a list of facts in the fact set such that all the terms from the list occur in the list of facts. -/
+theorem list_of_facts_for_list_of_terms {ts : List (GroundTerm sig)} {fs : FactSet sig} (ts_sub : ts.toSet ⊆ fs.terms) :
+    ∃ (l : List (Fact sig)), l.toSet ⊆ fs ∧ ts ⊆ l.flatMap GeneralizedAtom.terms := by
+  induction ts with
+  | nil => exists []; constructor; intro _ mem; simp [List.mem_toSet] at mem; simp
+  | cons t ts ih =>
+    rcases (ts_sub t (by simp [List.mem_toSet])) with ⟨f, f_mem, t_mem⟩
+    rcases ih (by intro _ mem; rw [List.mem_toSet] at mem; apply ts_sub; simp [List.mem_toSet, mem]) with ⟨l, l_sub, ts_sub⟩
+    exists (f :: l); constructor
+    . intro _ mem; rw [List.mem_toSet, List.mem_cons] at mem
+      cases mem with
+      | inl mem => rw [mem]; exact f_mem
+      | inr mem => apply l_sub; rw [List.mem_toSet]; exact mem
+    . intro s; rw [List.mem_cons, List.flatMap_cons, List.mem_append]
+      intro s_mem; cases s_mem with
+      | inl s_mem => apply Or.inl; rw [s_mem]; exact t_mem
+      | inr s_mem => apply Or.inr; apply ts_sub; exact s_mem
 
 end FactSet
 
+end FactSet
+
+section Database
+
+/-!
+## Database
+-/
+
+/-- A `Database` is a finite set of `FunctionFreeFact`s. -/
+abbrev Database (sig : Signature) [DecidableEq sig.P] [DecidableEq sig.C] [DecidableEq sig.V] := { X : Set (FunctionFreeFact sig) // X.finite }
+
 namespace Database
 
-  def constants (db : Database sig) : { C : Set sig.C // C.finite } := ⟨
-    fun c => ∃ (f : FunctionFreeFact sig), f ∈ db.val ∧ c ∈ f.terms,
-    by
-      rcases db.property with ⟨l, _, l_eq⟩
-      exists (l.flatMap (fun f => f.terms)).eraseDupsKeepRight
-      constructor
-      . apply List.nodup_eraseDupsKeepRight
-      . intro c
-        rw [List.mem_eraseDupsKeepRight, List.mem_flatMap]
-        constructor
-        . intro h
-          rcases h with ⟨f, f_mem, c_mem⟩
-          exists f
-          constructor
-          . rw [l_eq] at f_mem
-            exact f_mem
-          . exact c_mem
-        . intro h
-          rcases h with ⟨f, f_mem, c_mem⟩
-          exists f
-          constructor
-          . rw [← l_eq] at f_mem
-            exact f_mem
-          . exact c_mem
-  ⟩
+variable {sig : Signature} [DecidableEq sig.P] [DecidableEq sig.C] [DecidableEq sig.V]
 
-  def toFactSet (db : Database sig) : { fs : FactSet sig // fs.finite ∧ fs.isFunctionFree } := ⟨
-    (fun f => ∃ f', f' ∈ db.val ∧ f'.toFact = f),
-    (by
-      rcases db.property with ⟨l, _, l_eq⟩
-      exists (l.map FunctionFreeFact.toFact).eraseDupsKeepRight
-      constructor
-      . apply List.nodup_eraseDupsKeepRight
-      . intro f
-        rw [List.mem_eraseDupsKeepRight]
-        rw [List.mem_map]
-        simp only [l_eq]
-        rfl
-    ),
-    (by
-      intro f f_mem
-      rcases f_mem with ⟨_, _, f_eq⟩
-      rw [← f_eq]
-      apply FunctionFreeFact.toFact_isFunctionFree
-    ),
-  ⟩
-
-  theorem toFactSet_constants_same (db : Database sig) : db.toFactSet.val.constants = db.constants.val := by
-    unfold toFactSet
-    unfold constants
-    unfold FactSet.constants
-    simp only
-    apply Set.ext
-    intro c
+/-- Any `Database` can trivially be converted to a finite and function free `FactSet`. -/
+def toFactSet (db : Database sig) : { fs : FactSet sig // fs.finite ∧ fs.isFunctionFree } := ⟨
+  (fun f => ∃ f', f' ∈ db.val ∧ f'.toFact = f),
+  (by
+    rcases db.property with ⟨l, _, l_eq⟩
+    exists (l.map FunctionFreeFact.toFact).eraseDupsKeepRight
     constructor
-    . intro h
-      rcases h with ⟨f, f_mem, c_mem⟩
-      rcases f_mem with ⟨f', f'_mem, f_eq⟩
-      exists f'
+    . apply List.nodup_eraseDupsKeepRight
+    . intro f
+      rw [List.mem_eraseDupsKeepRight]
+      rw [List.mem_map]
+      simp only [l_eq]
+      rfl
+  ),
+  (by
+    intro f f_mem
+    rcases f_mem with ⟨_, _, f_eq⟩
+    rw [← f_eq]
+    apply FunctionFreeFact.toFact_isFunctionFree
+  ),
+⟩
+
+/-- Each `Database` has a finite set of constants. -/
+def constants (db : Database sig) : { C : Set sig.C // C.finite } := ⟨
+  fun c => ∃ (f : FunctionFreeFact sig), f ∈ db.val ∧ c ∈ f.terms,
+  by
+    rcases db.property with ⟨l, _, l_eq⟩
+    exists (l.flatMap (fun f => f.terms)).eraseDupsKeepRight
+    constructor
+    . apply List.nodup_eraseDupsKeepRight
+    . intro c
+      rw [List.mem_eraseDupsKeepRight, List.mem_flatMap]
       constructor
-      . exact f'_mem
-      . unfold Fact.constants at c_mem
-        rw [List.mem_flatMap] at c_mem
-        rcases c_mem with ⟨t, t_mem, c_mem⟩
-        rw [← f_eq] at t_mem
-        unfold FunctionFreeFact.toFact at t_mem
-        rw [List.mem_map] at t_mem
-        rcases t_mem with ⟨d, d_mem, t_eq⟩
-        rw [← t_eq] at c_mem
-        rw [GroundTerm.constants_const, List.mem_singleton] at c_mem
-        rw [c_mem]
-        exact d_mem
-    . intro h
-      rcases h with ⟨f, f_mem, c_mem⟩
-      exists f.toFact
-      constructor
-      . exists f
-      . unfold FunctionFreeFact.toFact
-        unfold Fact.constants
-        rw [List.mem_flatMap]
-        exists GroundTerm.const c
+      . intro h
+        rcases h with ⟨f, f_mem, c_mem⟩
+        exists f
         constructor
-        . rw [List.mem_map]
-          exists c
-        . simp [GroundTerm.constants_const]
+        . rw [l_eq] at f_mem
+          exact f_mem
+        . exact c_mem
+      . intro h
+        rcases h with ⟨f, f_mem, c_mem⟩
+        exists f
+        constructor
+        . rw [← l_eq] at f_mem
+          exact f_mem
+        . exact c_mem
+⟩
+
+/-- When converting a `Database` to a `FactSet`, the constants remain the same. -/
+theorem toFactSet_constants_same (db : Database sig) : db.toFactSet.val.constants = db.constants.val := by
+  unfold toFactSet
+  unfold constants
+  unfold FactSet.constants
+  simp only
+  apply Set.ext
+  intro c
+  constructor
+  . intro h
+    rcases h with ⟨f, f_mem, c_mem⟩
+    rcases f_mem with ⟨f', f'_mem, f_eq⟩
+    exists f'
+    constructor
+    . exact f'_mem
+    . unfold Fact.constants at c_mem
+      rw [List.mem_flatMap] at c_mem
+      rcases c_mem with ⟨t, t_mem, c_mem⟩
+      rw [← f_eq] at t_mem
+      unfold FunctionFreeFact.toFact at t_mem
+      rw [List.mem_map] at t_mem
+      rcases t_mem with ⟨d, d_mem, t_eq⟩
+      rw [← t_eq] at c_mem
+      rw [GroundTerm.constants_const, List.mem_singleton] at c_mem
+      rw [c_mem]
+      exact d_mem
+  . intro h
+    rcases h with ⟨f, f_mem, c_mem⟩
+    exists f.toFact
+    constructor
+    . exists f
+    . unfold FunctionFreeFact.toFact
+      unfold Fact.constants
+      rw [List.mem_flatMap]
+      exists GroundTerm.const c
+      constructor
+      . rw [List.mem_map]
+        exists c
+      . simp [GroundTerm.constants_const]
 
 end Database
+
+end Database
+
+section KnowledgeBase
+
+/-!
+## KnowledgeBase
+-/
+
+/-- A `KnowledgeBase` is a pair of a `Database` and a `RuleSet`. Note that usually the `RuleSet` is enforced to be finite but we only restrict this in places where we really need this. -/
+structure KnowledgeBase (sig : Signature) [DecidableEq sig.P] [DecidableEq sig.C] [DecidableEq sig.V] where
+  db : Database sig
+  rules : RuleSet sig
+
+namespace KnowledgeBase
+
+variable {sig : Signature} [DecidableEq sig.P] [DecidableEq sig.C] [DecidableEq sig.V]
+
+/-- A `KnowledgeBase` is determinstic if the underlying `RuleSet` is. -/
+def isDeterministic (kb : KnowledgeBase sig) : Prop := kb.rules.isDeterministic
+
+end KnowledgeBase
+
+end KnowledgeBase
 
