ExistentialRules/AtomsAndFacts/SubstitutionsAndHomomorphisms.lean
@@ -2,288 +2,357 @@ import BasicLeanDatastructures.List.Basic
 
 import ExistentialRules.AtomsAndFacts.Basic
 
-section Defs
+/-!
+# Substitutions and other mappings on Terms
 
-  abbrev TermMapping (S : Type u) (T : Type v) := S -> T
+In this file, we define mainly `GroundSubstitution` and `GroundTermMapping`. The latter is used to define homomorphisms on `FactSet`s.
+Both kinds of mapping are based on a (very general) `TermMapping`.
+-/
 
-  variable (sig : Signature) [DecidableEq sig.P] [DecidableEq sig.C] [DecidableEq sig.V]
+section TermMapping
 
-  abbrev GroundSubstitution := TermMapping sig.V (GroundTerm sig)
+/-!
+## TermMapping
 
-  abbrev GroundTermMapping := TermMapping (GroundTerm sig) (GroundTerm sig)
+The `TermMapping` is really just a function between two types but we
+define a bit of machinery on it that captures how remapping terms in such a general way behaves in the context of a `GeneralizedAtom` or lists or sets thereof.
+-/
 
-end Defs
+/-- A `TermMapping` is nothing more than a function from one term type to another. -/
+abbrev TermMapping (S : Type u) (T : Type v) := S -> T
 
 namespace TermMapping
 
-  variable {sig : Signature} [DecidableEq sig.P]
+variable {sig : Signature} [DecidableEq sig.P]
 
-  def apply_generalized_atom (h : TermMapping S T) (a : GeneralizedAtom sig S) : GeneralizedAtom sig T := {
-    predicate := a.predicate
-    terms := a.terms.map h
-    arity_ok := by rw [List.length_map, a.arity_ok]
-  }
+/-- A `TermMapping` is applied to a `GeneralizedAtom` by simply applying it to each term. -/
+def apply_generalized_atom (h : TermMapping S T) (a : GeneralizedAtom sig S) : GeneralizedAtom sig T := {
+  predicate := a.predicate
+  terms := a.terms.map h
+  arity_ok := by rw [List.length_map, a.arity_ok]
+}
 
-  theorem length_terms_apply_generalized_atom (h : TermMapping S T) (a : GeneralizedAtom sig S) :
-      (h.apply_generalized_atom a).terms.length = a.terms.length := by
-    simp [apply_generalized_atom]
+/-- A `TermMapping` is applied to a list of `GeneralizedAtom`s by applying it to each atom. -/
+def apply_generalized_atom_list (h : TermMapping S T) (l : List (GeneralizedAtom sig S)) : List (GeneralizedAtom sig T) :=
+  l.map h.apply_generalized_atom
 
-  theorem apply_generalized_atom_compose (g : TermMapping S T) (h : TermMapping T U) : apply_generalized_atom (sig := sig) (h ∘ g) = (apply_generalized_atom h) ∘ (apply_generalized_atom g) := by
-    apply funext
-    intro a
-    simp [apply_generalized_atom]
+/-- A `TermMapping` is applied to a set of `GeneralizedAtom`s by applying it to each atom. -/
+def apply_generalized_atom_set (h : TermMapping S T) (s : Set (GeneralizedAtom sig S)) : Set (GeneralizedAtom sig T) :=
+  s.map h.apply_generalized_atom
 
-  theorem apply_generalized_atom_compose' (g : TermMapping S T) (h : TermMapping T U) : ∀ (a : GeneralizedAtom sig S), apply_generalized_atom (h ∘ g) a = (apply_generalized_atom h) (apply_generalized_atom g a) := by
-    intro a
-    rw [← Function.comp_apply (f := h.apply_generalized_atom)]
-    rw [← apply_generalized_atom_compose]
+/-- Applying a `TermMapping` to a `GeneralizedAtom` does not change the number of terms.-/
+theorem length_terms_apply_generalized_atom (h : TermMapping S T) (a : GeneralizedAtom sig S) :
+    (h.apply_generalized_atom a).terms.length = a.terms.length := by
+  simp [apply_generalized_atom]
 
-  theorem apply_generalized_atom_congr_left (g h : TermMapping S T) (a : GeneralizedAtom sig S) : (∀ t ∈ a.terms, g t = h t) -> g.apply_generalized_atom a = h.apply_generalized_atom a := by
-    intro same
-    rw [GeneralizedAtom.mk.injEq]
+/-- We can split the application of a composed `TermMapping` on an atom. -/
+theorem apply_generalized_atom_compose (g : TermMapping S T) (h : TermMapping T U) : apply_generalized_atom (sig := sig) (h ∘ g) = (apply_generalized_atom h) ∘ (apply_generalized_atom g) := by
+  apply funext
+  intro a
+  simp [apply_generalized_atom]
+
+/-- We can split the application of a composed `TermMapping` on an atom. -/
+theorem apply_generalized_atom_compose' (g : TermMapping S T) (h : TermMapping T U) : ∀ (a : GeneralizedAtom sig S), apply_generalized_atom (h ∘ g) a = (apply_generalized_atom h) (apply_generalized_atom g a) := by
+  intro a
+  rw [← Function.comp_apply (f := h.apply_generalized_atom)]
+  rw [← apply_generalized_atom_compose]
+
+/-- To show that applying two `TermMapping`s on the same atom yields the same result, it is enough to show that the mappings behave identical on each term. -/
+theorem apply_generalized_atom_congr_left (g h : TermMapping S T) (a : GeneralizedAtom sig S) :
+    (∀ t ∈ a.terms, g t = h t) -> g.apply_generalized_atom a = h.apply_generalized_atom a := by
+  intro same
+  rw [GeneralizedAtom.mk.injEq]
+  constructor
+  . rfl
+  . apply List.map_congr_left
+    exact same
+
+/-- Applying a `TermMapping` on a `GeneralizedAtom` is the identity if the mapping is the identity on each term. -/
+theorem apply_generalized_atom_eq_self_of_id_on_terms (h : TermMapping T T) (a : GeneralizedAtom sig T) (id_on_terms : ∀ t ∈ a.terms, h t = t) :
+    h.apply_generalized_atom a = a := by
+  rw [GeneralizedAtom.mk.injEq]
+  constructor
+  . rfl
+  . apply List.map_id_of_id_on_all_mem
+    exact id_on_terms
+
+/-- We can split the application of a composed `TermMapping` on a list of atoms. -/
+theorem apply_generalized_atom_list_compose (g : TermMapping S T) (h : TermMapping T U) : apply_generalized_atom_list (sig := sig) (h ∘ g) = (apply_generalized_atom_list h) ∘ (apply_generalized_atom_list g) := by
+  apply funext
+  intro l
+  unfold apply_generalized_atom_list
+  rw [Function.comp_apply, List.map_map]
+  rw [apply_generalized_atom_compose]
+
+/-- We can split the application of a composed `TermMapping` on a list of atoms. -/
+theorem apply_generalized_atom_list_compose' (g : TermMapping S T) (h : TermMapping T U) : ∀ l : List (GeneralizedAtom sig S), apply_generalized_atom_list (h ∘ g) l = (apply_generalized_atom_list h) (apply_generalized_atom_list g l) := by
+  intro l
+  rw [← Function.comp_apply (f := h.apply_generalized_atom_list)]
+  rw [← apply_generalized_atom_list_compose]
+
+/-- We can split the application of a composed `TermMapping` on a set of atoms. -/
+theorem apply_generalized_atom_set_compose (g : TermMapping S T) (h : TermMapping T U) : apply_generalized_atom_set (sig := sig) (h ∘ g) = (apply_generalized_atom_set h) ∘ (apply_generalized_atom_set g) := by
+  apply funext
+  intro s
+  apply Set.ext
+  intro a
+  constructor
+  . intro pre
+    rcases pre with ⟨a', a'_mem, a'_eq⟩
+    rw [apply_generalized_atom_compose, Function.comp_apply] at a'_eq
+    exists g.apply_generalized_atom a'
     constructor
-    . rfl
-    . apply List.map_congr_left
-      exact same
-
-  theorem apply_generalized_atom_eq_self_of_id_on_terms (h : TermMapping T T) (a : GeneralizedAtom sig T) (id_on_terms : ∀ t ∈ a.terms, h t = t) : h.apply_generalized_atom a = a := by
-    rw [GeneralizedAtom.mk.injEq]
+    . exists a'
+    . exact a'_eq
+  . intro pre
+    rcases pre with ⟨a', a'_mem, a'_eq⟩
+    rcases a'_mem with ⟨a'', a''_mem, a''_eq⟩
+    exists a''
     constructor
-    . rfl
-    . apply List.map_id_of_id_on_all_mem
-      exact id_on_terms
+    . exact a''_mem
+    . rw [apply_generalized_atom_compose, Function.comp_apply]
+      rw [a'_eq, a''_eq]
 
-  def apply_generalized_atom_list (h : TermMapping S T) (l : List (GeneralizedAtom sig S)) : List (GeneralizedAtom sig T) :=
-    l.map h.apply_generalized_atom
+/-- We can split the application of a composed `TermMapping` on a set of atoms. -/
+theorem apply_generalized_atom_set_compose' (g : TermMapping S T) (h : TermMapping T U) : ∀ s : Set (GeneralizedAtom sig S), apply_generalized_atom_set (h ∘ g) s = (apply_generalized_atom_set h) (apply_generalized_atom_set g s) := by
+  intro l
+  rw [← Function.comp_apply (f := h.apply_generalized_atom_set)]
+  rw [← apply_generalized_atom_set_compose]
 
-  theorem apply_generalized_atom_list_compose (g : TermMapping S T) (h : TermMapping T U) : apply_generalized_atom_list (sig := sig) (h ∘ g) = (apply_generalized_atom_list h) ∘ (apply_generalized_atom_list g) := by
-    apply funext
-    intro l
-    unfold apply_generalized_atom_list
-    rw [Function.comp_apply, List.map_map]
-    rw [apply_generalized_atom_compose]
+/-- Applying a `TermMapping` to both an atom and a set of atoms retains membership of the atom in the set. -/
+theorem apply_generalized_atom_mem_apply_generalized_atom_set
+    (h : TermMapping S T) (a : GeneralizedAtom sig S) (as : Set (GeneralizedAtom sig S)) :
+    a ∈ as -> h.apply_generalized_atom a ∈ h.apply_generalized_atom_set as := by
+  intro a_mem
+  exists a
 
-  theorem apply_generalized_atom_list_compose' (g : TermMapping S T) (h : TermMapping T U) : ∀ l : List (GeneralizedAtom sig S), apply_generalized_atom_list (h ∘ g) l = (apply_generalized_atom_list h) (apply_generalized_atom_list g l) := by
-    intro l
-    rw [← Function.comp_apply (f := h.apply_generalized_atom_list)]
-    rw [← apply_generalized_atom_list_compose]
+/-- Applying the same `TermMapping` to two sets of atoms retains their subset relation. -/
+theorem apply_generalized_atom_set_subset_of_subset (h : TermMapping S T) (as bs : Set (GeneralizedAtom sig S)) :
+    as ⊆ bs -> h.apply_generalized_atom_set as ⊆ h.apply_generalized_atom_set bs := by
+  intro subset
+  intro a a_mem
+  rcases a_mem with ⟨a', a'_mem, a'_eq⟩
+  rw [a'_eq]
+  apply apply_generalized_atom_mem_apply_generalized_atom_set
+  apply subset
+  exact a'_mem
 
-  def apply_generalized_atom_set (h : TermMapping S T) (s : Set (GeneralizedAtom sig S)) : Set (GeneralizedAtom sig T) :=
-    s.map h.apply_generalized_atom
-
-  theorem apply_generalized_atom_set_compose (g : TermMapping S T) (h : TermMapping T U) : apply_generalized_atom_set (sig := sig) (h ∘ g) = (apply_generalized_atom_set h) ∘ (apply_generalized_atom_set g) := by
-    apply funext
-    intro s
-    apply Set.ext
-    intro a
-    constructor
-    . intro pre
-      rcases pre with ⟨a', a'_mem, a'_eq⟩
-      rw [apply_generalized_atom_compose, Function.comp_apply] at a'_eq
-      exists g.apply_generalized_atom a'
-      constructor
-      . exists a'
-      . exact a'_eq
-    . intro pre
-      rcases pre with ⟨a', a'_mem, a'_eq⟩
-      rcases a'_mem with ⟨a'', a''_mem, a''_eq⟩
-      exists a''
-      constructor
-      . exact a''_mem
-      . rw [apply_generalized_atom_compose, Function.comp_apply]
-        rw [a'_eq, a''_eq]
-
-  theorem apply_generalized_atom_set_compose' (g : TermMapping S T) (h : TermMapping T U) : ∀ s : Set (GeneralizedAtom sig S), apply_generalized_atom_set (h ∘ g) s = (apply_generalized_atom_set h) (apply_generalized_atom_set g s) := by
-    intro l
-    rw [← Function.comp_apply (f := h.apply_generalized_atom_set)]
-    rw [← apply_generalized_atom_set_compose]
-
-  theorem apply_generalized_atom_mem_apply_generalized_atom_set
-      (h : TermMapping S T) (a : GeneralizedAtom sig S) (as : Set (GeneralizedAtom sig S)) :
-      a ∈ as -> h.apply_generalized_atom a ∈ h.apply_generalized_atom_set as := by
-    intro a_mem
-    exists a
-
-  theorem apply_generalized_atom_set_subset_of_subset (h : TermMapping S T) (as bs : Set (GeneralizedAtom sig S)) :
-      as ⊆ bs -> h.apply_generalized_atom_set as ⊆ h.apply_generalized_atom_set bs := by
-    intro subset
-    intro a a_mem
-    rcases a_mem with ⟨a', a'_mem, a'_eq⟩
-    rw [a'_eq]
-    apply apply_generalized_atom_mem_apply_generalized_atom_set
-    apply subset
-    exact a'_mem
-
-  theorem apply_generalized_atom_set_toSet {g : TermMapping S T} : ∀ l : List (GeneralizedAtom sig S), g.apply_generalized_atom_set l.toSet = (g.apply_generalized_atom_list l).toSet := by
-    intro l; apply Set.ext; intro f; constructor
-    . rintro ⟨f', f'_mem, f_eq⟩; rw [f_eq, List.mem_toSet]; apply List.mem_map_of_mem; rw [← List.mem_toSet]; exact f'_mem
-    . simp only [List.mem_toSet, apply_generalized_atom_list, List.mem_map]; rintro ⟨f', f'_mem, f_eq⟩; rw [← f_eq]; apply apply_generalized_atom_mem_apply_generalized_atom_set; rw [List.mem_toSet]; exact f'_mem
+/-- When mapping a set of atoms that results from the list, we can instead map on the list and then convert to the set. -/
+theorem apply_generalized_atom_set_toSet {g : TermMapping S T} :
+    ∀ l : List (GeneralizedAtom sig S), g.apply_generalized_atom_set l.toSet = (g.apply_generalized_atom_list l).toSet := by
+  intro l; exact List.map_toSet_eq_toSet_map
 
 end TermMapping
 
+end TermMapping
+
+section GroundSubstitution
+
+/-!
+## GroundSubstitution
+
+`GroundSubstitution` is used mainly on rules to map the variables to some actual ground terms.
+This is a key ingredient of `PrTrigger`s that model "rule applications" in the chase.
+-/
+
+/-- A `GroundSubstitution` is merely a `TermMapping` from variables to `GroundTerm`s. -/
+abbrev GroundSubstitution (sig : Signature) [DecidableEq sig.C] [DecidableEq sig.V] := TermMapping sig.V (GroundTerm sig)
+
 namespace GroundSubstitution
 
-  variable {sig : Signature} [DecidableEq sig.C] [DecidableEq sig.V]
+variable {sig : Signature} [DecidableEq sig.C] [DecidableEq sig.V]
 
-  -- TODO: maybe rename this one and alike to lift_to_var_or_const
-  def apply_var_or_const (σ : GroundSubstitution sig) : TermMapping (VarOrConst sig) (GroundTerm sig)
-    | .var v => σ v
-    | .const c => GroundTerm.const c
+/-- We lift `GroundSubstitution`s to mappings from `VarOrConst` to `GroundTerm` in the obvious way. -/
+def apply_var_or_const (σ : GroundSubstitution sig) : TermMapping (VarOrConst sig) (GroundTerm sig)
+  | .var v => σ v
+  | .const c => GroundTerm.const c
 
-  def apply_skolem_term (σ : GroundSubstitution sig) : TermMapping (SkolemTerm sig) (GroundTerm sig)
-    | .var v => σ v
-    | .const c => GroundTerm.const c
-    | .func fs frontier arity_ok =>
-      GroundTerm.func fs (frontier.map (fun fv => σ fv)) (by
-        rw [List.length_map]
-        exact arity_ok
-      )
+/-- We lift `GroundSubstitution`s to mappings from `SkolemTerm` to `GroundTerm` in the obvious way. -/
+def apply_skolem_term (σ : GroundSubstitution sig) : TermMapping (SkolemTerm sig) (GroundTerm sig)
+  | .var v => σ v
+  | .const c => GroundTerm.const c
+  | .func fs frontier arity_ok =>
+    GroundTerm.func fs (frontier.map (fun fv => σ fv)) (by
+      rw [List.length_map]
+      exact arity_ok
+    )
 
-  theorem apply_skolem_term_injective_on_func_of_frontier_eq
-      (subs : GroundSubstitution sig) (s t : SkolemTerm sig)
-      (hs : s = SkolemTerm.func a frontier arity_a) (ht : t = SkolemTerm.func b frontier arity_b) :
-      subs.apply_skolem_term s = subs.apply_skolem_term t -> s = t := by
-    simp only [hs, ht, apply_skolem_term]
-    intro h
-    unfold GroundTerm.func at h
-    simp at h
-    simp [h]
+/-- On functional `SkolemTerm`s that share the same frontier, applying a `GroundSubstitution` is injective. -/
+theorem apply_skolem_term_injective_on_func_of_frontier_eq
+    (subs : GroundSubstitution sig) (s t : SkolemTerm sig)
+    (hs : s = SkolemTerm.func a frontier arity_a) (ht : t = SkolemTerm.func b frontier arity_b) :
+    subs.apply_skolem_term s = subs.apply_skolem_term t -> s = t := by
+  simp only [hs, ht, apply_skolem_term]
+  intro h
+  simp only [GroundTerm.func, Subtype.mk.injEq, FiniteTree.inner.injEq, and_true] at h
+  simp [h]
 
+variable [DecidableEq sig.P]
 
-  variable [DecidableEq sig.P]
+/-- Using the standard functionality of `TermMapping`, we can apply `GroundSubstitution`s directly to an `Atom` yielding a `Fact`. -/
+abbrev apply_atom (σ : GroundSubstitution sig) : Atom sig -> Fact sig :=
+  σ.apply_skolem_term.apply_generalized_atom
 
-  abbrev apply_atom (σ : GroundSubstitution sig) : Atom sig -> Fact sig :=
-    σ.apply_skolem_term.apply_generalized_atom
+/-- Using the standard functionality of `TermMapping`, we can apply `GroundSubstitution`s directly to a `FunctionFreeAtom` yielding a `Fact`. -/
+abbrev apply_function_free_atom (σ : GroundSubstitution sig) : FunctionFreeAtom sig -> Fact sig :=
+  σ.apply_var_or_const.apply_generalized_atom
 
-  abbrev apply_function_free_atom (σ : GroundSubstitution sig) : FunctionFreeAtom sig -> Fact sig :=
-    σ.apply_var_or_const.apply_generalized_atom
-
-  abbrev apply_function_free_conj (σ : GroundSubstitution sig) : FunctionFreeConjunction sig -> List (Fact sig) :=
-    σ.apply_var_or_const.apply_generalized_atom_list
+/-- Using the standard functionality of `TermMapping`, we can apply `GroundSubstitution`s directly to a `FunctionFreeConjunction` yielding a list of `Fact`s. -/
+abbrev apply_function_free_conj (σ : GroundSubstitution sig) : FunctionFreeConjunction sig -> List (Fact sig) :=
+  σ.apply_var_or_const.apply_generalized_atom_list
 
 end GroundSubstitution
 
+end GroundSubstitution
+
+section GroundTermMapping
+
+/-!
+## GroundTermMapping
+
+A `GroundTermMapping` maps `GroundTerm`s to `GroundTerm`s and is used to define homomorphisms over `FactSet`s.
+-/
+
+/-- A `GroundTermMapping` is merely a `TermMapping` over `GroundTerm`s. -/
+abbrev GroundTermMapping (sig : Signature) [DecidableEq sig.C] [DecidableEq sig.V] := TermMapping (GroundTerm sig) (GroundTerm sig)
 
 namespace GroundTermMapping
 
-  variable {sig : Signature} [DecidableEq sig.C] [DecidableEq sig.V]
+variable {sig : Signature} [DecidableEq sig.C] [DecidableEq sig.V]
 
-  def isIdOnConstants (h : GroundTermMapping sig) : Prop := ∀ {c}, h (.const c) = .const c
+def isIdOnConstants (h : GroundTermMapping sig) : Prop := ∀ {c}, h (.const c) = .const c
 
-  theorem apply_constant_is_id_of_isIdOnConstants {h : GroundTermMapping sig} (isId : h.isIdOnConstants) (c : sig.C) :
-      h (GroundTerm.const c) = GroundTerm.const c := isId
+variable [DecidableEq sig.P]
 
-  variable [DecidableEq sig.P]
+/-- Using the standard functionality of `TermMapping`, we can list `GroundTermMapping`s to `Fact`s. -/
+abbrev applyFact (h : GroundTermMapping sig) : Fact sig -> Fact sig := h.apply_generalized_atom
 
-  abbrev applyFact (h : GroundTermMapping sig) : Fact sig -> Fact sig := h.apply_generalized_atom
+/-- Using the standard functionality of `TermMapping`, we can list `GroundTermMapping`s to `FactSet`s. -/
+abbrev applyFactSet (h : GroundTermMapping sig) : FactSet sig -> FactSet sig := h.apply_generalized_atom_set
 
-  abbrev applyFactSet (h : GroundTermMapping sig) : FactSet sig -> FactSet sig := h.apply_generalized_atom_set
+/-- A `GroundTermMapping` is a homomorphisms from `FactSet` A to B if each constant is mapped to itself and mapping A results in a subset of B. -/
+def isHomomorphism (h : GroundTermMapping sig) (A B : FactSet sig) : Prop :=
+  isIdOnConstants h ∧ (h.applyFactSet A ⊆ B)
 
-  theorem terms_applyFactSet {h : GroundTermMapping sig} {fs : FactSet sig} : (h.applyFactSet fs).terms = fs.terms.map h := by
-    apply Set.ext; intro t
+/-- The terms in a mapped `FactSet` are the same as the mapped terms from the original `FactSet`. -/
+theorem terms_applyFactSet {h : GroundTermMapping sig} {fs : FactSet sig} : (h.applyFactSet fs).terms = fs.terms.map h := by
+  apply Set.ext; intro t
+  constructor
+  . rintro ⟨f, ⟨f', f'_mem, f_eq⟩, t_mem⟩
+    rw [f_eq] at t_mem
+    simp only [TermMapping.apply_generalized_atom, List.mem_map] at t_mem
+    rcases t_mem with ⟨t', t'_mem, t_eq⟩
+    rw [← t_eq]
+    exists t'; simp only [and_true]
+    exists f'
+  . rintro ⟨t', ⟨f', f'_mem, t'_mem⟩, t_eq⟩
+    rw [t_eq]
+    exists h.applyFact f'; constructor
+    . apply TermMapping.apply_generalized_atom_mem_apply_generalized_atom_set; exact f'_mem
+    . simp only [applyFact, TermMapping.apply_generalized_atom]; apply List.mem_map_of_mem; exact t'_mem
+
+/-- We can compose homomorphisms. That is, given a homomorphism from A to B and from B to C, we can combine both to obtain a homomorphisms from A to C. -/
+theorem isHomomorphism_compose (g h : GroundTermMapping sig) (A B C : FactSet sig) :
+    g.isHomomorphism A B -> h.isHomomorphism B C -> isHomomorphism (h ∘ g) A C := by
+  intro g_hom h_hom
+  constructor
+  . intro c
+    rw [Function.comp_apply, g_hom.left, h_hom.left]
+  . unfold applyFactSet
+    rw [TermMapping.apply_generalized_atom_set_compose]
+    intro f f_mem_compose
+    rcases f_mem_compose with ⟨f', f'_mem, f'_eq⟩
+    apply h_hom.right
+    exists f'
     constructor
-    . rintro ⟨f, ⟨f', f'_mem, f_eq⟩, t_mem⟩
-      rw [f_eq] at t_mem
-      simp only [TermMapping.apply_generalized_atom, List.mem_map] at t_mem
-      rcases t_mem with ⟨t', t'_mem, t_eq⟩
-      rw [← t_eq]
-      exists t'; simp only [and_true]
-      exists f'
-    . rintro ⟨t', ⟨f', f'_mem, t'_mem⟩, t_eq⟩
-      rw [t_eq]
-      exists h.applyFact f'; constructor
-      . apply TermMapping.apply_generalized_atom_mem_apply_generalized_atom_set; exact f'_mem
-      . simp only [applyFact, TermMapping.apply_generalized_atom]; apply List.mem_map_of_mem; exact t'_mem
+    . apply g_hom.right
+      exact f'_mem
+    . exact f'_eq
 
-  def isHomomorphism (h : GroundTermMapping sig) (A B : FactSet sig) : Prop :=
-    isIdOnConstants h ∧ (h.applyFactSet A ⊆ B)
-
-  theorem isHomomorphism_compose (g h : GroundTermMapping sig) (A B C : FactSet sig) :
-      g.isHomomorphism A B -> h.isHomomorphism B C -> isHomomorphism (h ∘ g) A C := by
-    intro g_hom h_hom
-    constructor
-    . intro c
-      rw [Function.comp_apply, g_hom.left, h_hom.left]
-    . unfold applyFactSet
-      rw [TermMapping.apply_generalized_atom_set_compose]
-      intro f f_mem_compose
-      rcases f_mem_compose with ⟨f', f'_mem, f'_eq⟩
-      apply h_hom.right
-      exists f'
-      constructor
-      . apply g_hom.right
-        exact f'_mem
-      . exact f'_eq
+end GroundTermMapping
 
 end GroundTermMapping
 
 section GroundSubstitutionInteractionWithGroundTermMapping
 
-  variable {sig : Signature} [DecidableEq sig.C] [DecidableEq sig.V]
+/-!
+## Interactions of GroundSubstitution and GroundTermMapping
 
-  theorem GroundSubstitution.apply_var_or_const_compose (s : GroundSubstitution sig) (h : GroundTermMapping sig) :
-      ∀ (voc : VarOrConst sig), (∀ d, voc = VarOrConst.const d -> h (GroundTerm.const d) = GroundTerm.const d) -> GroundSubstitution.apply_var_or_const (h ∘ s) voc = h (s.apply_var_or_const voc) := by
-    intro voc id_on_const
-    unfold GroundSubstitution.apply_var_or_const
-    cases voc with
-    | var v => simp
-    | const c =>
-      simp only
-      rw [id_on_const]
-      rfl
+Sometimes, a `GroundSubstitution` and `GroundTermMapping` might be composed into a single `GroundSubstitution`.
+In such a case, it can be useful to be able to split them apart. But this is generally only possible if the `GroundTermMapping` leaves the relevant constants untouched.
+-/
 
-  theorem GroundSubstitution.apply_var_or_const_compose_of_isIdOnConstants (s : GroundSubstitution sig)
-      (h : GroundTermMapping sig) (id_on_const : h.isIdOnConstants) :
-      GroundSubstitution.apply_var_or_const (h ∘ s) = h ∘ s.apply_var_or_const := by
-    apply funext
-    intro voc
-    apply apply_var_or_const_compose
-    intros
-    exact id_on_const
+variable {sig : Signature} [DecidableEq sig.C] [DecidableEq sig.V]
 
-  variable [DecidableEq sig.P]
+/-- The application of a composed substitution on a `VarOrConst` can be split if the involved `GroundTermMapping` maps the `VarOrConst` to itself, in the case where it is a constant. -/
+theorem GroundSubstitution.apply_var_or_const_compose (s : GroundSubstitution sig) (h : GroundTermMapping sig) :
+    ∀ (voc : VarOrConst sig), (∀ d, voc = VarOrConst.const d -> h (GroundTerm.const d) = GroundTerm.const d) -> GroundSubstitution.apply_var_or_const (h ∘ s) voc = h (s.apply_var_or_const voc) := by
+  intro voc id_on_const
+  unfold GroundSubstitution.apply_var_or_const
+  cases voc with
+  | var v => simp
+  | const c =>
+    simp only
+    rw [id_on_const]
+    rfl
 
-  theorem GroundSubstitution.apply_function_free_atom_compose (s : GroundSubstitution sig) (h : GroundTermMapping sig) :
-      ∀ (a : FunctionFreeAtom sig), (∀ d ∈ a.constants, h (GroundTerm.const d) = GroundTerm.const d) -> GroundSubstitution.apply_function_free_atom (h ∘ s) a = h.applyFact (s.apply_function_free_atom a) := by
-    intro a id_on_const
-    unfold GroundTermMapping.applyFact
-    rw [← TermMapping.apply_generalized_atom_compose']
-    apply TermMapping.apply_generalized_atom_congr_left
-    intro voc voc_mem
-    apply apply_var_or_const_compose
-    intro d d_eq
-    apply id_on_const
-    unfold FunctionFreeAtom.constants
-    apply VarOrConst.mem_filterConsts_of_const
-    rw [d_eq] at voc_mem
-    exact voc_mem
+/-- This is a special case of the above theorem where the `GroundTermMapping` is simply the id on all constants. -/
+theorem GroundSubstitution.apply_var_or_const_compose_of_isIdOnConstants (s : GroundSubstitution sig)
+    (h : GroundTermMapping sig) (id_on_const : h.isIdOnConstants) :
+    GroundSubstitution.apply_var_or_const (h ∘ s) = h ∘ s.apply_var_or_const := by
+  apply funext
+  intro voc
+  apply apply_var_or_const_compose
+  intros
+  exact id_on_const
 
-  theorem GroundSubstitution.apply_function_free_atom_compose_of_isIdOnConstants (s : GroundSubstitution sig) (h : GroundTermMapping sig) (id_on_const : h.isIdOnConstants) :
-      GroundSubstitution.apply_function_free_atom (h ∘ s) = h.applyFact ∘ s.apply_function_free_atom := by
-    apply funext
-    intro a
-    apply apply_function_free_atom_compose
-    intros
-    exact id_on_const
+variable [DecidableEq sig.P]
 
-  theorem GroundSubstitution.apply_function_free_conj_compose (s : GroundSubstitution sig) (h : GroundTermMapping sig) :
-      ∀ (ffc : FunctionFreeConjunction sig), (∀ d ∈ ffc.consts, h (GroundTerm.const d) = GroundTerm.const d) -> GroundSubstitution.apply_function_free_conj (h ∘ s) ffc = h.apply_generalized_atom_list (s.apply_function_free_conj ffc) := by
-    intro ffc id_on_const
-    unfold GroundSubstitution.apply_function_free_conj TermMapping.apply_generalized_atom_list
-    rw [List.map_map]
-    apply List.map_congr_left
-    intro f f_mem
-    rw [← apply_function_free_atom.eq_def, apply_function_free_atom_compose]
-    . rfl
-    . intro d d_mem; apply id_on_const; simp only [FunctionFreeConjunction.consts, List.mem_flatMap]; exists f
+/-- The application of a composed substitution on a `FunctionFreeAtom` can be split if the involved `GroundTermMapping` maps all constants from the atom to themselves. -/
+theorem GroundSubstitution.apply_function_free_atom_compose (s : GroundSubstitution sig) (h : GroundTermMapping sig) :
+    ∀ (a : FunctionFreeAtom sig), (∀ d ∈ a.constants, h (GroundTerm.const d) = GroundTerm.const d) -> GroundSubstitution.apply_function_free_atom (h ∘ s) a = h.applyFact (s.apply_function_free_atom a) := by
+  intro a id_on_const
+  unfold GroundTermMapping.applyFact
+  rw [← TermMapping.apply_generalized_atom_compose']
+  apply TermMapping.apply_generalized_atom_congr_left
+  intro voc voc_mem
+  apply apply_var_or_const_compose
+  intro d d_eq
+  apply id_on_const
+  unfold FunctionFreeAtom.constants
+  apply VarOrConst.mem_filterConsts_of_const
+  rw [d_eq] at voc_mem
+  exact voc_mem
 
-  theorem GroundSubstitution.apply_function_free_conj_compose_of_isIdOnConstants (s : GroundSubstitution sig) (h : GroundTermMapping sig) (id_on_const : h.isIdOnConstants) :
-      GroundSubstitution.apply_function_free_conj (h ∘ s) = h.apply_generalized_atom_list ∘ s.apply_function_free_conj := by
-    apply funext
-    intro ffc
-    apply apply_function_free_conj_compose
-    intros
-    exact id_on_const
+/-- This is a special case of the above theorem where the `GroundTermMapping` is simply the id on all constants. -/
+theorem GroundSubstitution.apply_function_free_atom_compose_of_isIdOnConstants (s : GroundSubstitution sig) (h : GroundTermMapping sig) (id_on_const : h.isIdOnConstants) :
+    GroundSubstitution.apply_function_free_atom (h ∘ s) = h.applyFact ∘ s.apply_function_free_atom := by
+  apply funext
+  intro a
+  apply apply_function_free_atom_compose
+  intros
+  exact id_on_const
+
+/-- The application of a composed substitution on a `FunctionFreeConjunction` can be split if the involved `GroundTermMapping` maps all constants from the conjucntion to themselves. -/
+theorem GroundSubstitution.apply_function_free_conj_compose (s : GroundSubstitution sig) (h : GroundTermMapping sig) :
+    ∀ (ffc : FunctionFreeConjunction sig), (∀ d ∈ ffc.consts, h (GroundTerm.const d) = GroundTerm.const d) -> GroundSubstitution.apply_function_free_conj (h ∘ s) ffc = h.apply_generalized_atom_list (s.apply_function_free_conj ffc) := by
+  intro ffc id_on_const
+  unfold GroundSubstitution.apply_function_free_conj TermMapping.apply_generalized_atom_list
+  rw [List.map_map]
+  apply List.map_congr_left
+  intro f f_mem
+  rw [← apply_function_free_atom.eq_def, apply_function_free_atom_compose]
+  . rfl
+  . intro d d_mem; apply id_on_const; simp only [FunctionFreeConjunction.consts, List.mem_flatMap]; exists f
+
+/-- This is a special case of the above theorem where the `GroundTermMapping` is simply the id on all constants. -/
+theorem GroundSubstitution.apply_function_free_conj_compose_of_isIdOnConstants (s : GroundSubstitution sig) (h : GroundTermMapping sig) (id_on_const : h.isIdOnConstants) :
+    GroundSubstitution.apply_function_free_conj (h ∘ s) = h.apply_generalized_atom_list ∘ s.apply_function_free_conj := by
+  apply funext
+  intro ffc
+  apply apply_function_free_conj_compose
+  intros
+  exact id_on_const
 
 end GroundSubstitutionInteractionWithGroundTermMapping
 
